moving some code around, improved compositional memory symbolic evaluator.

src/SymIL.v
@@ -5,8 +5,9 @@ Require Import IL SepIL.
 Require Import Word Memory.
 Require Import DepList EqdepClass.
 Require Import PropX.
-Require Expr SepExpr.
-Require Import Provers.
+Require Import SepExpr SymEval.
+Require Import Expr.
+Require Import Prover.
 Require Import Env.
 Import List.
 
@@ -60,230 +61,223 @@ Definition bedrock_types : list Expr.type :=
     in repr bedrock_types_r nil.
 
 (** Symbolic Evaluation **)
-Module PLUGIN := SymEval.EvaluatorPlugin BedrockHeap ST.
+Module MEVAL := SymEval.MemoryEvaluator BedrockHeap ST.
+Module SEP := MEVAL.SEP.
 
-Module BedrockEvaluator.
-  Require Import SepExpr SymEval.
-  Require Import Expr.
-
-  Module SEP := PLUGIN.SEP.
-
-
-  Section SymState.
-    Variable types : list type.
-    Variables pcT stT : tvar.
+Section SymState.
+  Variable types : list type.
+  Variables pcT stT : tvar.
 
     (** Symbolic registers **)
-    Definition SymRegType : Type :=
-      (expr types * expr types * expr types)%type.
+  Definition SymRegType : Type :=
+    (expr types * expr types * expr types)%type.
 
     (** Symbolic State **)
-    Record SymState : Type :=
+  Record SymState : Type :=
     { SymVars  : variables
-    ; SymUVars : variables
-    ; SymMem   : option (SEP.SHeap types pcT stT)
-    ; SymRegs  : SymRegType
-    ; SymPures : list (expr types)
+      ; SymUVars : variables
+      ; SymMem   : option (SEP.SHeap types pcT stT)
+      ; SymRegs  : SymRegType
+      ; SymPures : list (expr types)
     }.
 
     (** Register accessor functions **)
-    Definition sym_getReg (r : reg) (sr : SymRegType) : expr types :=
-      match r with
-        | Sp => fst (fst sr)
-        | Rp => snd (fst sr)
-        | Rv => snd sr
-      end.
+  Definition sym_getReg (r : reg) (sr : SymRegType) : expr types :=
+    match r with
+      | Sp => fst (fst sr)
+      | Rp => snd (fst sr)
+      | Rv => snd sr
+    end.
 
-    Definition sym_setReg (r : reg) (v : expr types) (sr : SymRegType) : SymRegType :=
-      match r with
-        | Sp => (v, snd (fst sr), snd sr)
-        | Rp => (fst (fst sr), v, snd sr)
-        | Rv => (fst sr, v)
-      end.
-  End SymState.
+  Definition sym_setReg (r : reg) (v : expr types) (sr : SymRegType) : SymRegType :=
+    match r with
+      | Sp => (v, snd (fst sr), snd sr)
+      | Rp => (fst (fst sr), v, snd sr)
+      | Rv => (fst sr, v)
+    end.
+End SymState.
 
-  Section typed.
-    Context {types : list type}.
-   
+Section typed.
+  Context {types : list type}.
+  
     (** These the reflected version of the IL, it essentially 
      ** replaces all uses of W with expr types so that the value
      ** can be inspected.
      **)
-    Inductive sym_loc :=
-    | SymReg : reg -> sym_loc
-    | SymImm : expr types -> sym_loc
-    | SymIndir : reg -> expr types -> sym_loc.
+  Inductive sym_loc :=
+  | SymReg : reg -> sym_loc
+  | SymImm : expr types -> sym_loc
+  | SymIndir : reg -> expr types -> sym_loc.
 
     (* Valid targets of assignments *)
-    Inductive sym_lvalue :=
-    | SymLvReg : reg -> sym_lvalue
-    | SymLvMem : sym_loc -> sym_lvalue.
-    
+  Inductive sym_lvalue :=
+  | SymLvReg : reg -> sym_lvalue
+  | SymLvMem : sym_loc -> sym_lvalue.
+  
     (* Operands *)
-    Inductive sym_rvalue :=
-    | SymRvLval : sym_lvalue -> sym_rvalue
-    | SymRvImm : expr types -> sym_rvalue
-    | SymRvLabel : label -> sym_rvalue.
+  Inductive sym_rvalue :=
+  | SymRvLval : sym_lvalue -> sym_rvalue
+  | SymRvImm : expr types -> sym_rvalue
+  | SymRvLabel : label -> sym_rvalue.
 
     (* Non-control-flow instructions *)
-    Inductive sym_instr :=
-    | SymAssign : sym_lvalue -> sym_rvalue -> sym_instr
-    | SymBinop : sym_lvalue -> sym_rvalue -> binop -> sym_rvalue -> sym_instr.
+  Inductive sym_instr :=
+  | SymAssign : sym_lvalue -> sym_rvalue -> sym_instr
+  | SymBinop : sym_lvalue -> sym_rvalue -> binop -> sym_rvalue -> sym_instr.
 
-    Inductive sym_assert :=
-    | SymAssertCond : sym_rvalue -> test -> sym_rvalue -> option bool -> sym_assert.
-    (** NOTE : I can use something like this to generate intermediate states
-    | SymCheckPoint : expr types -> sym_assert.
-    **)
+  Inductive sym_assert :=
+  | SymAssertCond : sym_rvalue -> test -> sym_rvalue -> option bool -> sym_assert.
 
-  End typed.
+End typed.
 
-  Implicit Arguments sym_loc [ ].
-  Implicit Arguments sym_lvalue [ ].
-  Implicit Arguments sym_rvalue [ ].
-  Implicit Arguments sym_instr [ ].
-  Implicit Arguments sym_assert [ ].
+Implicit Arguments sym_loc [ ].
+Implicit Arguments sym_lvalue [ ].
+Implicit Arguments sym_rvalue [ ].
+Implicit Arguments sym_instr [ ].
+Implicit Arguments sym_assert [ ].
 
-  Definition comparator (t : IL.test) (l r : W) : Prop :=
-    match t with
-      | IL.Eq => l = r
-      | IL.Ne => l = r -> False
-      | IL.Lt => wlt l r
-      | IL.Le => wlt l r \/ l = r
+Definition comparator (t : IL.test) (l r : W) : Prop :=
+  match t with
+    | IL.Eq => l = r
+    | IL.Ne => l = r -> False
+    | IL.Lt => wlt l r
+    | IL.Le => wlt l r \/ l = r
+  end.
+
+Section typed_ext.
+  Variable types' : list type.
+  Local Notation "'TYPES'" := (repr bedrock_types_r types').
+
+  Local Notation "'pcT'" := (tvType 0).
+  Local Notation "'tvWord'" := (tvType 0).
+  Local Notation "'stT'" := (tvType 1).
+  Local Notation "'tvState'" := (tvType 2).
+  Local Notation "'tvTest'" := (tvType 3).
+  Local Notation "'tvReg'" := (tvType 4).
+
+  Definition bedrock_funcs_r : Repr (signature (repr bedrock_types_r types')).
+  refine (
+    {| default := Default_signature _
+      ; footprint := (
+        (0, {| Domain := tvWord :: tvWord :: nil
+          ; Range := tvWord
+          ; Denotation := _ |}) ::
+        (1, {| Domain := tvWord :: tvWord :: nil
+          ; Range := tvWord
+          ; Denotation := _ |}) ::
+        (2, {| Domain := tvWord :: tvWord :: nil
+          ; Range := tvWord
+          ; Denotation := _ |}) ::
+        (3, {| Domain := tvTest :: tvWord :: tvWord :: nil
+          ; Range := tvProp
+          ; Denotation := _ |}) :: 
+        (4, {| Domain := tvState :: tvReg :: nil
+          ; Range := tvWord
+          ; Denotation := _ |}) :: nil) :: nil
+    |});
+  cbv beta iota zeta delta [ functionTypeD map ]; (repeat rewrite tvarD_repr_repr_get); simpl.
+  refine (@wplus 32).
+  refine (@wminus 32).
+  refine (@wmult 32).
+  refine comparator.
+  refine Regs.
+  Defined.
+
+  Definition bedrock_funcs : functions (repr bedrock_types_r types') :=
+    Eval cbv beta iota zeta delta 
+      [ repr repr' default footprint fold_right bedrock_funcs_r updateAt hd_error error value
+        bedrock_types_r Default_signature tl hd ]
+      in repr bedrock_funcs_r nil.
+  
+  Variable funcs' : functions TYPES.
+  Definition funcs := repr bedrock_funcs_r funcs'.
+  
+  Definition fPlus (l r : expr TYPES) : expr TYPES :=
+    Expr.Func 0 (l :: r :: nil).
+  Definition fMinus (l r : expr TYPES) : expr TYPES :=
+    Expr.Func 1 (l :: r :: nil).
+  Definition fMult (l r : expr TYPES) : expr TYPES :=
+    Expr.Func 2 (l :: r :: nil).
+
+  Theorem fPlus_correct : forall l r uvars vars, 
+    match exprD funcs uvars vars l (tvType 0) , exprD funcs uvars vars r (tvType 0) with
+      | Some lv , Some rv =>
+        exprD funcs uvars vars (fPlus l r) (tvType 0) = Some (wplus lv rv)
+      | _ , _ => True
+    end.
+  Proof.
+    intros; simpl; unfold eq_ind_r; simpl;
+      repeat match goal with
+               | [ |- match ?X with
+                        | Some _ => _
+                        | None => _
+                      end ] => destruct X
+             end; auto.
+  Qed.
+  Theorem fMinus_correct : forall l r uvars vars, 
+    match exprD funcs uvars vars l tvWord , exprD funcs uvars vars r tvWord with
+      | Some lv , Some rv =>
+        exprD funcs uvars vars (fMinus l r) tvWord = Some (wminus lv rv)
+      | _ , _ => True
+    end.
+  Proof.
+    intros; simpl; unfold eq_ind_r; simpl;
+      repeat match goal with
+               | [ |- match ?X with
+                        | Some _ => _
+                        | None => _
+                      end ] => destruct X
+             end; auto.
+  Qed.
+  Theorem fMult_correct : forall l r uvars vars, 
+    match exprD funcs uvars vars l tvWord , exprD funcs uvars vars r tvWord with
+      | Some lv , Some rv =>
+        exprD funcs uvars vars (fMult l r) tvWord = Some (wmult lv rv)
+      | _ , _ => True
+    end.
+  Proof.
+    intros; simpl; unfold eq_ind_r; simpl;
+      repeat match goal with
+               | [ |- match ?X with
+                        | Some _ => _
+                        | None => _
+                      end ] => destruct X
+             end; auto.
+  Qed.
+
+  Variable Prover : ProverT TYPES.
+
+  (** these are the plugin functions **)
+  Variable symeval_read_word :
+    Facts Prover -> expr TYPES -> SEP.SHeap TYPES pcT stT 
+    -> option (expr TYPES).
+  Variable symeval_write_word :
+    Facts Prover -> expr TYPES -> expr TYPES -> SEP.SHeap TYPES pcT stT 
+    -> option (SEP.SHeap TYPES pcT stT).
+
+  (** This has to be connected to the type of the intermediate representation **)
+  Definition sym_evalLoc (lv : sym_loc TYPES) (ss : SymState TYPES pcT stT) : expr TYPES :=
+    match lv with
+      | SymReg r => sym_getReg r (SymRegs ss)
+      | SymImm l => l
+      | SymIndir r w => fPlus (sym_getReg r (SymRegs ss)) w
     end.
 
-  Section typed_ext.
-    Variable types' : list type.
-    Definition types := repr bedrock_types_r types'.
+Section with_facts.
+  Variable Facts : Facts Prover.
 
-    Local Notation "'pcT'" := (tvType 0).
-    Local Notation "'tvWord'" := (tvType 0).
-    Local Notation "'stT'" := (tvType 1).
-    Local Notation "'tvState'" := (tvType 2).
-    Local Notation "'tvTest'" := (tvType 3).
-    Local Notation "'tvReg'" := (tvType 4).
-
-    Definition bedrock_funcs_r : Repr (signature (repr bedrock_types_r types')).
-    refine (
-      {| default := Default_signature _
-        ; footprint := (
-          (0, {| Domain := tvWord :: tvWord :: nil
-            ; Range := tvWord
-            ; Denotation := _ |}) ::
-          (1, {| Domain := tvWord :: tvWord :: nil
-            ; Range := tvWord
-            ; Denotation := _ |}) ::
-          (2, {| Domain := tvWord :: tvWord :: nil
-            ; Range := tvWord
-            ; Denotation := _ |}) ::
-          (3, {| Domain := tvTest :: tvWord :: tvWord :: nil
-            ; Range := tvProp
-            ; Denotation := _ |}) :: 
-          (4, {| Domain := tvState :: tvReg :: nil
-            ; Range := tvWord
-            ; Denotation := _ |}) :: nil) :: nil
-      |});
-    cbv beta iota zeta delta [ functionTypeD map ]; (repeat rewrite tvarD_repr_repr_get); simpl.
-    refine (@wplus 32).
-    refine (@wminus 32).
-    refine (@wmult 32).
-    refine comparator.
-    refine Regs.
-    Defined.
-
-    Definition bedrock_funcs : functions (repr bedrock_types_r types') :=
-      Eval cbv beta iota zeta delta 
-        [ repr repr' default footprint fold_right bedrock_funcs_r updateAt hd_error error value
-          bedrock_types_r Default_signature tl hd ]
-        in repr bedrock_funcs_r nil.
-
-    Variable funcs' : functions types.
-    Definition funcs := repr bedrock_funcs_r funcs'.
-
-    Definition fPlus (l r : expr types) : expr types :=
-      Expr.Func 0 (l :: r :: nil).
-    Definition fMinus (l r : expr types) : expr types :=
-      Expr.Func 1 (l :: r :: nil).
-    Definition fMult (l r : expr types) : expr types :=
-      Expr.Func 2 (l :: r :: nil).
-
-    Theorem fPlus_correct : forall l r uvars vars, 
-      match exprD funcs uvars vars l (tvType 0) , exprD funcs uvars vars r (tvType 0) with
-        | Some lv , Some rv =>
-          exprD funcs uvars vars (fPlus l r) (tvType 0) = Some (wplus lv rv)
-        | _ , _ => True
-      end.
-    Proof.
-      intros; simpl; unfold eq_ind_r; simpl;
-      repeat match goal with
-               | [ |- match ?X with
-                        | Some _ => _
-                        | None => _
-                      end ] => destruct X
-             end; auto.
-   Qed.
-    Theorem fMinus_correct : forall l r uvars vars, 
-      match exprD funcs uvars vars l tvWord , exprD funcs uvars vars r tvWord with
-        | Some lv , Some rv =>
-          exprD funcs uvars vars (fMinus l r) tvWord = Some (wminus lv rv)
-        | _ , _ => True
-      end.
-    Proof.
-      intros; simpl; unfold eq_ind_r; simpl;
-      repeat match goal with
-               | [ |- match ?X with
-                        | Some _ => _
-                        | None => _
-                      end ] => destruct X
-             end; auto.
-    Qed.
-    Theorem fMult_correct : forall l r uvars vars, 
-      match exprD funcs uvars vars l tvWord , exprD funcs uvars vars r tvWord with
-        | Some lv , Some rv =>
-          exprD funcs uvars vars (fMult l r) tvWord = Some (wmult lv rv)
-        | _ , _ => True
-      end.
-    Proof.
-      intros; simpl; unfold eq_ind_r; simpl;
-      repeat match goal with
-               | [ |- match ?X with
-                        | Some _ => _
-                        | None => _
-                      end ] => destruct X
-             end; auto.
-    Qed.
-
-    Variable Prover : ProverT types.
-
-    (** these are the plugin functions **)
-    Variable symeval_read_word : Facts Prover -> expr types -> SEP.SHeap types pcT stT 
-      -> option (expr types).
-    Variable symeval_write_word : Facts Prover -> expr types -> expr types -> SEP.SHeap types pcT stT 
-      -> option (SEP.SHeap types pcT stT).
-    
-    (** This has to be connected to the type of the intermediate representation **)
-    Definition sym_evalLoc (lv : sym_loc types) (ss : SymState types pcT stT) : expr types :=
-      match lv with
-        | SymReg r => sym_getReg r (SymRegs ss)
-        | SymImm l => l
-        | SymIndir r w => fPlus (sym_getReg r (SymRegs ss)) w
-      end.
-
-    Section with_facts.
-    Variable Facts : Facts Prover.
-
-    Definition sym_evalLval (lv : sym_lvalue types) (val : expr types) (ss : SymState types pcT stT)
-      : option (SymState types pcT stT) :=
-      match lv with
-        | SymLvReg r =>
-          Some {| SymVars := SymVars ss
-                ; SymUVars := SymUVars ss
-                ; SymMem := SymMem ss 
-                ; SymRegs := sym_setReg r val (SymRegs ss)
-                ; SymPures := SymPures ss
-                |}
-        | SymLvMem l => 
-          let l := sym_evalLoc l ss in
+  Definition sym_evalLval (lv : sym_lvalue TYPES) (val : expr TYPES) (ss : SymState TYPES pcT stT)
+    : option (SymState TYPES pcT stT) :=
+    match lv with
+      | SymLvReg r =>
+        Some {| SymVars := SymVars ss
+              ; SymUVars := SymUVars ss
+              ; SymMem := SymMem ss 
+              ; SymRegs := sym_setReg r val (SymRegs ss)
+              ; SymPures := SymPures ss
+              |}
+      | SymLvMem l => 
+        let l := sym_evalLoc l ss in
           match SymMem ss with
             | None => None
             | Some m =>
@@ -298,9 +292,9 @@ Module BedrockEvaluator.
                 | None => None
               end
           end
-      end.
+    end.
 
-    Definition sym_evalRval (rv : sym_rvalue types) (ss : SymState types pcT stT) : option (expr types) :=
+    Definition sym_evalRval (rv : sym_rvalue TYPES) (ss : SymState TYPES pcT stT) : option (expr TYPES) :=
       match rv with
         | SymRvLval (SymLvReg r) =>
           Some (sym_getReg r (SymRegs ss))
@@ -316,11 +310,11 @@ Module BedrockEvaluator.
         (* an alternative would be to reflect these as a function call that does the positioning...
          * - it isn't clear that this can be done since the environment would need to depend on the settings.
          *)
-        (*Some (Expr.Const (types := types) (t := tvType 2) l) *)
+        (*Some (Expr.Const (TYPES := TYPES) (t := tvType 2) l) *)
       end.
 
-    Definition sym_assertTest (r : sym_rvalue types) (t : test) (l : sym_rvalue types) (ss : SymState types pcT stT) (res : bool) 
-      : option (expr types) :=
+    Definition sym_assertTest (r : sym_rvalue TYPES) (t : test) (l : sym_rvalue TYPES) (ss : SymState TYPES pcT stT) (res : bool) 
+      : option (expr TYPES) :=
       let '(l, t, r) := if res
         then (l, t, r)
         else match t with
@@ -333,12 +327,12 @@ Module BedrockEvaluator.
         | Some l , Some r =>
           match t with
             | IL.Eq => Some (Expr.Equal tvWord l r)
-            | _ => Some (Expr.Func 3 (Expr.Const (types := types) (t := tvTest) t :: l :: r :: nil))
+            | _ => Some (Expr.Func 3 (Expr.Const (types := TYPES) (t := tvTest) t :: l :: r :: nil))
           end
         | _ , _ => None
       end.
 
-    Definition sym_evalInstr (i : sym_instr types) (ss : SymState types pcT stT) : option (SymState types pcT stT) :=
+    Definition sym_evalInstr (i : sym_instr TYPES) (ss : SymState TYPES pcT stT) : option (SymState TYPES pcT stT) :=
       match i with 
         | SymAssign lv rv =>
           match sym_evalRval rv ss with
@@ -360,8 +354,8 @@ Module BedrockEvaluator.
           end
       end.
 
-    Fixpoint sym_evalInstrs (is : list (sym_instr types)) (ss : SymState types pcT stT) 
-      : SymState types pcT stT + (SymState types pcT stT * list (sym_instr types)) :=
+    Fixpoint sym_evalInstrs (is : list (sym_instr TYPES)) (ss : SymState TYPES pcT stT) 
+      : SymState TYPES pcT stT + (SymState TYPES pcT stT * list (sym_instr TYPES)) :=
       match is with
         | nil => inl ss
         | i :: is =>
@@ -371,147 +365,135 @@ Module BedrockEvaluator.
           end
       end.
 
-    End with_facts.
+  End with_facts.
 
-    Definition istream : Type := list ((list (sym_instr types) * option state) + sym_assert types).
+  Definition istream : Type := list ((list (sym_instr TYPES) * option state) + sym_assert TYPES).
 
-    (** TODO: I need variables here in order to call the unfolder **)
-    Variable learnHook : forall P : ProverT types, SymState types pcT stT -> Facts P -> SymState types pcT stT.
+  Definition LearnHook (types_ : list type) (pcT_ stT_ : tvar) : Type := 
+    forall P : ProverT types_, SymState types_ pcT_ stT_ -> Facts P -> SymState types_ pcT_ stT_.
 
-    Fixpoint sym_evalStream (is : istream) (F : Facts Prover) (ss : SymState types pcT stT) 
-      : option (SymState types pcT stT) + (SymState types pcT stT * istream) :=
-      match is with
-        | nil => inl (Some ss)
-        | inl (ins, st) :: is =>
-          match sym_evalInstrs F ins ss with
-            | inr (ss,rm) => inr (ss, inl (rm, st) :: is)
-            | inl ss => sym_evalStream is F ss
-          end
-        | inr asrt :: is =>
-          match asrt with
-            | SymAssertCond l t r (Some res) =>
-              match sym_assertTest F l t r ss res with
-                | Some sp =>
-                  let F' := Learn Prover F (sp :: nil) in 
+  Variable learnHook : LearnHook TYPES pcT stT.
+
+  Fixpoint sym_evalStream (is : istream) (F : Facts Prover) (ss : SymState TYPES pcT stT) 
+    : option (SymState TYPES pcT stT) + (SymState TYPES pcT stT * istream) :=
+    match is with
+      | nil => inl (Some ss)
+      | inl (ins, st) :: is =>
+        match sym_evalInstrs F ins ss with
+          | inr (ss,rm) => inr (ss, inl (rm, st) :: is)
+          | inl ss => sym_evalStream is F ss
+        end
+      | inr asrt :: is =>
+        match asrt with
+          | SymAssertCond l t r (Some res) =>
+            match sym_assertTest F l t r ss res with
+              | Some sp =>
+                let F' := Learn Prover F (sp :: nil) in 
                   let ss' := 
                     {| SymVars := SymVars ss
-                     ; SymUVars := SymUVars ss
-                     ; SymRegs := SymRegs ss 
-                     ; SymMem := SymMem ss
-                     ; SymPures := sp :: SymPures ss
-                     |}
-                  in
-                  let ss' := learnHook Prover ss' F' in
-(*
-                  let facts' := Learn Prover (SymFacts ss) (sp :: nil) in
-                  (** TODO: perform unfolding here **)
-                  match learnHook 
-                  let mem' := SymMem ss in
-                  
-                  let ss' :=
-                    {| SumSymRegs := SymRegs ss 
-                     ; SymMem := mem' 
-                     ; SymPures := sp :: SymPures ss
-                     ; SymFacts := facts' 
-                     |}
-                  in
-*)
-                  sym_evalStream is F' ss'
-                | None => inr (ss, inr asrt :: is)
-              end
-            | SymAssertCond l t r None =>
-              match sym_evalRval F l ss , sym_evalRval F r ss with
-                | None , _ => inl None
-                | _ , None => inl None
-                | _ , _ => sym_evalStream is F ss 
-              end
+                      ; SymUVars := SymUVars ss
+                      ; SymRegs := SymRegs ss 
+                      ; SymMem := SymMem ss
+                      ; SymPures := sp :: SymPures ss
+                    |}
+                    in
+                    let ss' := learnHook Prover ss' F' in
+                    sym_evalStream is F' ss'
+              | None => inr (ss, inr asrt :: is)
+            end
+          | SymAssertCond l t r None =>
+            match sym_evalRval F l ss , sym_evalRval F r ss with
+              | None , _ => inl None
+              | _ , None => inl None
+              | _ , _ => sym_evalStream is F ss 
+            end
+        end
+    end.
+
+  (* Denotation functions *)
+  Section sym_denote.
+    Variable funcs : functions TYPES.
+    Variable uvars vars : env TYPES.
+    
+    Definition sym_regsD (rs : SymRegType TYPES) : option regs :=
+      match rs with
+        | (sp, rp, rv) =>
+          match 
+            exprD funcs uvars vars sp tvWord ,
+            exprD funcs uvars vars rp tvWord ,
+            exprD funcs uvars vars rv tvWord 
+            with
+            | Some sp , Some rp , Some rv =>
+              Some (fun r => 
+                match r with
+                  | Sp => sp
+                  | Rp => rp
+                  | Rv => rv
+                end)
+            | _ , _ , _ => None
           end
       end.
 
-    (* Denotation functions *)
-    Section sym_denote.
-      Variable funcs : functions types.
-      Variable uvars vars : env types.
+    Definition sym_locD (s : sym_loc TYPES) : option loc :=
+      match s with
+        | SymReg r => Some (Reg r)
+        | SymImm e =>
+          match exprD funcs uvars vars e tvWord with
+            | Some e => Some (Imm e)
+            | None => None
+          end
+        | SymIndir r o =>
+          match exprD funcs uvars vars o tvWord with
+            | Some o => Some (Indir r o)
+            | None => None
+          end
+      end.
 
-      Definition sym_regsD (rs : SymRegType types) : option regs :=
-        match rs with
-          | (sp, rp, rv) =>
-            match 
-              exprD funcs uvars vars sp tvWord ,
-              exprD funcs uvars vars rp tvWord ,
-              exprD funcs uvars vars rv tvWord 
-              with
-              | Some sp , Some rp , Some rv =>
-                Some (fun r => 
-                  match r with
-                    | Sp => sp
-                    | Rp => rp
-                    | Rv => rv
-                  end)
-              | _ , _ , _ => None
-            end
-        end.
+    Definition sym_lvalueD (s : sym_lvalue TYPES) : option lvalue :=
+      match s with
+        | SymLvReg r => Some (LvReg r)
+        | SymLvMem l => match sym_locD l with
+                          | Some l => Some (LvMem l)
+                          | None => None
+                        end
+      end.
 
-      Definition sym_locD (s : sym_loc types) : option loc :=
-        match s with
-          | SymReg r => Some (Reg r)
-          | SymImm e =>
-            match exprD funcs uvars vars e tvWord with
-              | Some e => Some (Imm e)
-              | None => None
-            end
-          | SymIndir r o =>
-            match exprD funcs uvars vars o tvWord with
-              | Some o => Some (Indir r o)
-              | None => None
-            end
-        end.
+    Definition sym_rvalueD (r : sym_rvalue TYPES) : option rvalue :=
+      match r with
+        | SymRvLval l => match sym_lvalueD l with
+                           | Some l => Some (RvLval l)
+                           | None => None
+                         end
+        | SymRvImm e => match exprD funcs uvars vars e tvWord with
+                          | Some l => Some (RvImm l)
+                          | None => None
+                        end
+        | SymRvLabel l => Some (RvLabel l)
+      end.
 
-      Definition sym_lvalueD (s : sym_lvalue types) : option lvalue :=
-        match s with
-          | SymLvReg r => Some (LvReg r)
-          | SymLvMem l => match sym_locD l with
-                            | Some l => Some (LvMem l)
-                            | None => None
-                          end
-        end.
+    Definition sym_instrD (i : sym_instr TYPES) : option instr :=
+      match i with
+        | SymAssign l r =>
+          match sym_lvalueD l , sym_rvalueD r with
+            | Some l , Some r => Some (Assign l r)
+            | _ , _ => None
+          end
+        | SymBinop lhs l o r =>
+          match sym_lvalueD lhs , sym_rvalueD l , sym_rvalueD r with
+            | Some lhs , Some l , Some r => Some (Binop lhs l o r)
+            | _ , _ , _ => None
+          end
+      end.
 
-      Definition sym_rvalueD (r : sym_rvalue types) : option rvalue :=
-        match r with
-          | SymRvLval l => match sym_lvalueD l with
-                             | Some l => Some (RvLval l)
-                             | None => None
-                           end
-          | SymRvImm e => match exprD funcs uvars vars e tvWord with
-                            | Some l => Some (RvImm l)
-                            | None => None
-                          end
-          | SymRvLabel l => Some (RvLabel l)
-        end.
-
-      Definition sym_instrD (i : sym_instr types) : option instr :=
-        match i with
-          | SymAssign l r =>
-            match sym_lvalueD l , sym_rvalueD r with
-              | Some l , Some r => Some (Assign l r)
-              | _ , _ => None
-            end
-          | SymBinop lhs l o r =>
-            match sym_lvalueD lhs , sym_rvalueD l , sym_rvalueD r with
-              | Some lhs , Some l , Some r => Some (Binop lhs l o r)
-              | _ , _ , _ => None
-            end
-        end.
-
-      Fixpoint sym_instrsD (is : list (sym_instr types)) : option (list instr) :=
-        match is with
-          | nil => Some nil
-          | i :: is => 
-            match sym_instrD i , sym_instrsD is with
-              | Some i , Some is => Some (i :: is)
-              | _ , _ => None
-            end
-        end.
+    Fixpoint sym_instrsD (is : list (sym_instr TYPES)) : option (list instr) :=
+      match is with
+        | nil => Some nil
+        | i :: is => 
+          match sym_instrD i , sym_instrsD is with
+            | Some i , Some is => Some (i :: is)
+            | _ , _ => None
+          end
+      end.
 
     Fixpoint istreamD (is : istream) (stn : settings) (st : state) (res : option state) : Prop :=
       match is with
@@ -541,147 +523,116 @@ Module BedrockEvaluator.
           end
       end.
 
-      Variable sfuncs : SEP.sfunctions types pcT stT.
+    Variable sfuncs : SEP.sfunctions TYPES pcT stT.
 
-      Definition stateD cs (stn : IL.settings) (s : state) (ss : SymState types pcT stT) : Prop :=
-        match ss with
-          | {| SymMem := m ; SymRegs := (sp, rp, rv) ; SymPures := pures |} =>
-            match 
-             exprD funcs uvars vars sp tvWord ,
-             exprD funcs uvars vars rp tvWord ,
-             exprD funcs uvars vars rv tvWord
-            with
-              | Some sp , Some rp , Some rv =>
-                Regs s Sp = sp /\ Regs s Rp = rp /\ Regs s Rv = rv
-              | _ , _ , _ => False
-            end
-            /\ match m with 
-                 | None => True
-                 | Some m => 
-                   PropX.interp cs (SepIL.SepFormula.sepFormula (SEP.sexprD funcs sfuncs uvars vars (SEP.sheapD m)) (stn, s))%PropX
-               end
-            /\ AllProvable funcs uvars vars pures 
-        end.
+    Definition stateD cs (stn : IL.settings) (s : state) (ss : SymState TYPES pcT stT) : Prop :=
+      match ss with
+        | {| SymMem := m ; SymRegs := (sp, rp, rv) ; SymPures := pures |} =>
+             match 
+               exprD funcs uvars vars sp tvWord ,
+               exprD funcs uvars vars rp tvWord ,
+               exprD funcs uvars vars rv tvWord
+               with
+               | Some sp , Some rp , Some rv =>
+                 Regs s Sp = sp /\ Regs s Rp = rp /\ Regs s Rv = rv
+               | _ , _ , _ => False
+             end
+          /\ match m with 
+               | None => True
+               | Some m => 
+                 PropX.interp cs (SepIL.SepFormula.sepFormula (SEP.sexprD funcs sfuncs uvars vars (SEP.sheapD m)) (stn, s))%PropX
+             end
+          /\ AllProvable funcs uvars vars pures 
+      end.
 
-      Lemma hash_interp : forall sfuncs se sh,
-        SEP.hash se = (nil, sh) ->
-        forall uvars vars st stn cs,
-          PropX.interp cs (![ @SEP.sexprD types funcs pcT stT sfuncs uvars vars se ] (stn, st)) ->
-          PropX.interp cs (![ @SEP.sexprD types funcs pcT stT sfuncs uvars vars (SEP.sheapD sh) ] (stn, st)).
-      Proof.
-        clear. intros.
-        generalize (SEP.hash_denote funcs sfuncs cs se uvars vars).
-        rewrite H. simpl. intros.
-        rewrite <- H1. eauto.
-      Qed.
-    End sym_denote.
-  End typed_ext.
+    Lemma hash_interp : forall sfuncs se sh,
+      SEP.hash se = (nil, sh) ->
+      forall uvars vars st stn cs,
+        PropX.interp cs (![ @SEP.sexprD TYPES funcs pcT stT sfuncs uvars vars se ] (stn, st)) ->
+        PropX.interp cs (![ @SEP.sexprD TYPES funcs pcT stT sfuncs uvars vars (SEP.sheapD sh) ] (stn, st)).
+    Proof.
+      clear. intros.
+      generalize (SEP.hash_denote funcs sfuncs cs se uvars vars).
+      rewrite H. simpl. intros.
+      rewrite <- H1. eauto.
+    Qed.
+  End sym_denote.
+End typed_ext.
 
-  Section evaluator.
-    Record SymEvaluator types (pcT stT : tvar) : Type :=
-    { symeval_read_word : forall (P : Provers.ProverT types), Provers.Facts P -> 
-      expr types -> SEP.SHeap types pcT stT -> option (expr types)
-    ; symeval_write_word : forall (P : Provers.ProverT types), Provers.Facts P ->
-      expr types -> expr types -> SEP.SHeap types pcT stT -> option (SEP.SHeap types pcT stT)
-    }.
+(** TODO: this needs to be abstracted to not talk about bedrock **)
+Record LearnHook_correct types' (L : LearnHook (repr bedrock_types_r types') (tvType 0) (tvType 1)) funcs preds : Prop :=
+{ hook_sound : forall P (PC : ProverT_correct P funcs),
+  forall uvars vars cs stn st ss ss' pp,
+    @stateD _ funcs uvars vars preds cs stn st ss ->
+    Valid PC uvars vars pp ->
+    L P ss pp = ss' ->
+    @stateD _ funcs uvars vars preds cs stn st ss'
+}.
 
-    Local Notation "'pcT'" := (tvType 0).
-    Local Notation "'tvWord'" := (tvType 0).
-    Local Notation "'stT'" := (tvType 1).
-    Local Notation "'tvState'" := (tvType 2).
-    Local Notation "'tvTest'" := (tvType 3).
-    Local Notation "'tvReg'" := (tvType 4).
+Section evaluator.
+  Variable types' : list type.
 
-    Record SymEvaluator_correct types'
-      (funcs : functions (repr bedrock_types_r types')) (preds : SEP.sfunctions (repr bedrock_types_r types') pcT stT) 
-      (Evaluator : SymEvaluator (repr bedrock_types_r types') (tvType 0) (tvType 1))
-      : Type :=
-    { ReadCorrect :
-      forall (P : Provers.ProverT (repr bedrock_types_r types')) (PE : Provers.ProverT_correct P funcs),
-        forall facts (pe ve : expr (repr bedrock_types_r types')) SH,
-          symeval_read_word Evaluator P facts pe SH = Some ve ->
-          forall uvars vars cs p m stn,
-            Provers.Valid PE uvars vars facts ->
-            exprD funcs uvars vars pe tvWord = Some p ->
-            PropX.interp cs (![ SEP.sexprD funcs preds uvars vars (SEP.sheapD SH) ] (stn, m)) ->
-            match exprD funcs uvars vars ve tvWord with
-              | Some v =>
-                ReadWord stn (Mem m) p = Some v
-              | _ => False
-            end
-    ; WriteCorrect :
-      forall (P : Provers.ProverT (repr bedrock_types_r types')) (PE : Provers.ProverT_correct P funcs),
-        forall uvars vars cs facts pe ve m stn SH SH',
-          symeval_write_word Evaluator P facts pe ve SH = Some SH' ->
-            Provers.Valid PE uvars vars facts ->
-            forall p v,
-            exprD funcs uvars vars pe tvWord = Some p ->
-            exprD funcs uvars vars ve tvWord = Some v ->
-            PropX.interp cs (![ SEP.sexprD funcs preds uvars vars (SEP.sheapD SH) ] (stn, m)) ->
-            match mem_set_word _ _ (footprint_w) (BedrockHeap.mem_set) (explode stn) p v (Mem m) with
-              | None => False
-              | Some m' =>
-                PropX.interp cs (![ SEP.sexprD funcs preds uvars vars (SEP.sheapD SH') ] (stn, {| Regs := Regs m ; Mem := m' |}))
-            end
-    }.
+  Local Notation "'pcT'" := (tvType 0).
+  Local Notation "'tvWord'" := (tvType 0).
+  Local Notation "'stT'" := (tvType 1).
+  Local Notation "'tvState'" := (tvType 2).
+  Local Notation "'tvTest'" := (tvType 3).
+  Local Notation "'tvReg'" := (tvType 4).
 
-    Definition LearnHook types : Type := 
-      forall P : Provers.ProverT types, SymState types pcT stT -> Provers.Facts P -> SymState types pcT stT.
+  Local Notation "'TYPES'" := (Env.repr bedrock_types_r types').
 
-    Record LearnHook_correct types' (L : LearnHook (types types')) funcs preds : Prop :=
-    { hook_sound : forall P (PC : ProverT_correct P funcs),
-      forall uvars vars cs stn st ss ss' pp,
-      @stateD _ funcs uvars vars preds cs stn st ss ->
-      Valid PC uvars vars pp ->
-      L P ss pp = ss' ->
-      @stateD _ funcs uvars vars preds cs stn st ss'
-    }.
+  Variable mem_eval : MEVAL.MemEvaluator TYPES pcT stT.
 
-    Theorem sym_eval_any : forall types',
-      let types := repr bedrock_types_r types' in
-      forall (funcs : functions types) (sfuncs : SEP.sfunctions types _ _),
-      forall E,  @SymEvaluator_correct types' funcs sfuncs E ->
-      forall P, Provers.ProverT_correct P funcs ->
-      forall L, @LearnHook_correct _ L funcs sfuncs ->
-      forall stn uvars vars sound_or_safe st p,
-        istreamD funcs uvars vars p stn st sound_or_safe ->
-        forall cs ss,
-        stateD funcs uvars vars sfuncs cs stn st ss ->
-        let facts := Summarize P (match SymMem ss with
-                                    | None => SymPures ss
-                                    | Some m => pures m
-                                  end) in
-        let res := @sym_evalStream _ P (symeval_read_word E P) (symeval_write_word E P) L p facts ss in
-        match sound_or_safe with
-          | None =>
+  Definition IL_stn_st : Type := (IL.settings * IL.state)%type.
+
+  Definition IL_mem_satisfies (cs : PropX.codeSpec (tvarD TYPES pcT) (tvarD TYPES stT)) 
+    (P : ST.hprop (tvarD TYPES pcT) (tvarD TYPES stT) nil) (stn_st : IL_stn_st) : Prop :=
+    PropX.interp cs (SepIL.SepFormula.sepFormula P stn_st).
+      
+  Definition IL_ReadWord : IL_stn_st -> tvarD TYPES tvWord -> option (tvarD TYPES tvWord) :=
+    (fun stn_st => IL.ReadWord (fst stn_st) (Mem (snd stn_st))).
+  Definition IL_WriteWord : IL_stn_st -> tvarD TYPES tvWord -> tvarD TYPES tvWord -> option IL_stn_st :=
+    (fun stn_st p v => 
+      let (stn,st) := stn_st in
+      match IL.WriteWord stn (Mem st) p v with
+        | None => None
+        | Some m => Some (stn, {| Regs := Regs st ; Mem := m |})
+      end).
+
+  Theorem sym_eval_any :     
+    forall (funcs : functions TYPES) (sfuncs : SEP.sfunctions TYPES _ _),
+    forall E, @MEVAL.MemEvaluator_correct TYPES _ _ E funcs sfuncs _ _ _ IL_mem_satisfies IL_ReadWord IL_WriteWord ->
+    forall P, ProverT_correct P funcs ->
+    forall L, @LearnHook_correct _ L funcs sfuncs ->
+    forall stn uvars vars sound_or_safe st p,
+      istreamD funcs uvars vars p stn st sound_or_safe ->
+      forall cs ss,
+      stateD funcs uvars vars sfuncs cs stn st ss ->
+      let facts := Summarize P (match SymMem ss with
+                                  | None => SymPures ss
+                                  | Some m => pures m
+                                end) in
+      let res := @sym_evalStream _ P (MEVAL.smemeval_read_word E P) (MEVAL.smemeval_write_word E P) L p facts ss in
+      match sound_or_safe with
+        | None =>
             (** safe **)
             match res with
               | inl None => True
               | inl (Some _) => False
-              | inr (ss'', is') => True (*
-                exists st'' : state,
-                  match sym_instrsD is' with
-                    | Some instrs' =>
-                      evalInstrs stn st'' instrs' = None /\
-                      stateD cs stn st'' ss''
-                    | None => False
-                  end
-*)
+              | inr (ss'', is') => 
+                exists st'' : state, 
+                  istreamD funcs uvars vars is' stn st'' None
+                  /\ stateD funcs uvars vars sfuncs cs stn st'' ss''
             end
           | Some st' =>
             (** correct **)
             match res with
               | inl None => False                
               | inl (Some ss') => stateD funcs uvars vars sfuncs cs stn st' ss'
-              | inr (ss'', is') => True (*
-                exists st'' : state,
-                  match sym_instrsD is' with
-                    | Some instrs' =>
-                      evalInstrs stn st'' instrs' = Some st' /\
-                      stateD cs stn st'' ss''
-                    | None => False
-                  end
-*)
+              | inr (ss'', is') => 
+                exists st'' : state, 
+                  istreamD funcs uvars vars is' stn st'' (Some st')
+                  /\ stateD funcs uvars vars sfuncs cs stn st'' ss''
             end
         end.
     Proof.
@@ -730,17 +681,16 @@ Module BedrockEvaluator.
       eexists. split. eassumption. eapply Imply_E. eapply H1. auto.
     Qed.
 
-    Theorem stateD_proof_no_heap types' : 
-      let types :=  repr bedrock_types_r types' in
-        forall (funcs : Expr.functions types) (P : ProverT types)
+    Theorem stateD_proof_no_heap :
+        forall (funcs : Expr.functions TYPES) (P : ProverT TYPES)
           (PC : ProverT_correct P funcs),
-          forall (uvars vars : Expr.env types)
-            (sfuncs : SEP.sfunctions types pcT stT) 
-            (st : state) (sp rv rp : Expr.expr types),
+          forall (uvars vars : Expr.env TYPES)
+            (sfuncs : SEP.sfunctions TYPES pcT stT) 
+            (st : state) (sp rv rp : Expr.expr TYPES),
             exprD funcs uvars vars sp tvWord = Some (Regs st Sp) ->
             exprD funcs uvars vars rv tvWord = Some (Regs st Rv) ->
             exprD funcs uvars vars rp tvWord = Some (Regs st Rp) ->
-            forall pures : list (Expr.expr types),
+            forall pures : list (Expr.expr TYPES),
               Expr.AllProvable funcs uvars vars pures ->
               forall (cs : codeSpec W (settings * state)) (stn : settings),
                 stateD funcs uvars vars sfuncs cs stn st
@@ -752,40 +702,37 @@ Module BedrockEvaluator.
                 |}.
     Proof.
       unfold stateD. intros.
-      unfold types.
       repeat match goal with
                | [ H : _ = _ |- _ ] => rewrite H
              end.
       intuition auto. 
     Qed.
 
-    Theorem stateD_proof types' : 
-      let types :=  repr bedrock_types_r types' in
-        forall (funcs : Expr.functions types) (P : ProverT types)
-          (PC : ProverT_correct P funcs),
-          forall (uvars vars : Expr.env types)
-            (sfuncs : SEP.sfunctions types pcT stT) 
-            (st : state) (sp rv rp : Expr.expr types),
-            exprD funcs uvars vars sp tvWord = Some (Regs st Sp) ->
-            exprD funcs uvars vars rv tvWord = Some (Regs st Rv) ->
-            exprD funcs uvars vars rp tvWord = Some (Regs st Rp) ->
-            forall pures : list (Expr.expr types),
-              Expr.AllProvable funcs uvars vars pures ->
-              forall (sh : SEP.sexpr types pcT stT)
-                (hashed : SEP.SHeap types pcT stT),
-                SEP.hash sh = (nil, hashed) ->
-                forall (cs : codeSpec W (settings * state)) (stn : settings),
-                  interp cs (![SEP.sexprD funcs sfuncs uvars vars sh] (stn, st)) ->
-                  stateD funcs uvars vars sfuncs cs stn st
-                  {| SymVars := map (@projT1 _ _) vars
-                   ; SymUVars := map (@projT1 _ _) uvars
-                   ; SymMem := Some hashed
-                   ; SymRegs := (sp, rp, rv)
-                   ; SymPures := pures
-                   |}.
+    Theorem stateD_proof :
+      forall (funcs : Expr.functions TYPES) (P : ProverT TYPES)
+        (PC : ProverT_correct P funcs),
+        forall (uvars vars : Expr.env TYPES)
+          (sfuncs : SEP.sfunctions TYPES pcT stT) 
+          (st : state) (sp rv rp : Expr.expr TYPES),
+          exprD funcs uvars vars sp tvWord = Some (Regs st Sp) ->
+          exprD funcs uvars vars rv tvWord = Some (Regs st Rv) ->
+          exprD funcs uvars vars rp tvWord = Some (Regs st Rp) ->
+          forall pures : list (Expr.expr TYPES),
+            Expr.AllProvable funcs uvars vars pures ->
+            forall (sh : SEP.sexpr TYPES pcT stT)
+              (hashed : SEP.SHeap TYPES pcT stT),
+              SEP.hash sh = (nil, hashed) ->
+              forall (cs : codeSpec W (settings * state)) (stn : settings),
+                interp cs (![SEP.sexprD funcs sfuncs uvars vars sh] (stn, st)) ->
+                stateD funcs uvars vars sfuncs cs stn st
+                {| SymVars := map (@projT1 _ _) vars
+                 ; SymUVars := map (@projT1 _ _) uvars
+                 ; SymMem := Some hashed
+                 ; SymRegs := (sp, rp, rv)
+                 ; SymPures := pures
+                 |}.
     Proof.
       unfold stateD. intros.
-      unfold types.
       repeat match goal with
                | [ H : _ = _ |- _ ] => rewrite H
              end.
@@ -794,144 +741,144 @@ Module BedrockEvaluator.
     Qed.
   End evaluator.
 
-  (** Reflection **)
+(** Reflection **)
 
-  (* Reflect the instructions *)
-  Ltac collectTypes_loc isConst l Ts :=
-    match l with
-      | Reg _ => Ts
-      | Imm ?i => collectTypes_expr isConst i Ts
-      | Indir _ ?i => collectTypes_expr isConst i Ts
-    end.
-  Ltac reify_loc isConst l types funcs uvars vars k :=
-    match l with
-      | Reg ?r => 
-        let res := constr:(@SymReg types r) in
+(* Reflect the instructions *)
+Ltac collectTypes_loc isConst l Ts :=
+  match l with
+    | Reg _ => Ts
+    | Imm ?i => collectTypes_expr isConst i Ts
+    | Indir _ ?i => collectTypes_expr isConst i Ts
+  end.
+Ltac reify_loc isConst l types funcs uvars vars k :=
+  match l with
+    | Reg ?r => 
+      let res := constr:(@SymReg types r) in
         k uvars funcs res
-      | Imm ?i =>
-        reify_expr isConst i types funcs uvars vars ltac:(fun uvars funcs i =>
-          let l := constr:(@SymImm types i) in k uvars funcs l)
-      | Indir ?r ?i =>
-        reify_expr isConst i types funcs uvars vars ltac:(fun uvars funcs i =>
-          let l := constr:(@SymIndir types r i) in k uvars funcs l)
-    end.
+    | Imm ?i =>
+      reify_expr isConst i types funcs uvars vars ltac:(fun uvars funcs i =>
+        let l := constr:(@SymImm types i) in k uvars funcs l)
+    | Indir ?r ?i =>
+      reify_expr isConst i types funcs uvars vars ltac:(fun uvars funcs i =>
+        let l := constr:(@SymIndir types r i) in k uvars funcs l)
+  end.
 
-  Ltac collectTypes_lvalue isConst l Ts :=
-    match l with
-      | LvReg _ => Ts
-      | LvMem ?l => collectTypes_loc isConst l Ts
-    end.
-  Ltac reify_lvalue isConst l types funcs uvars vars k :=
-    match l with
-      | LvReg ?r => let l := constr:(@SymLvReg types r) in k uvars funcs l 
-      | LvMem ?l => 
-        reify_loc isConst l types funcs uvars vars ltac:(fun uvars funcs l =>
-          let l := constr:(@SymLvMem types l) in k uvars funcs l)
-    end.
+Ltac collectTypes_lvalue isConst l Ts :=
+  match l with
+    | LvReg _ => Ts
+    | LvMem ?l => collectTypes_loc isConst l Ts
+  end.
+Ltac reify_lvalue isConst l types funcs uvars vars k :=
+  match l with
+    | LvReg ?r => let l := constr:(@SymLvReg types r) in k uvars funcs l 
+    | LvMem ?l => 
+      reify_loc isConst l types funcs uvars vars ltac:(fun uvars funcs l =>
+        let l := constr:(@SymLvMem types l) in k uvars funcs l)
+  end.
 
-  Ltac collectTypes_rvalue isConst r Ts :=
-    match r with
-      | RvLval ?l => collectTypes_lvalue isConst l Ts
-      | RvImm ?i => collectTypes_expr isConst i Ts
-      | RvLabel _ => let l := constr:(label:Type) in Reflect.cons_uniq l Ts
-    end.
+Ltac collectTypes_rvalue isConst r Ts :=
+  match r with
+    | RvLval ?l => collectTypes_lvalue isConst l Ts
+    | RvImm ?i => collectTypes_expr isConst i Ts
+    | RvLabel _ => let l := constr:(label:Type) in Reflect.cons_uniq l Ts
+  end.
 
-  Ltac reify_rvalue isConst r types funcs uvars vars k :=
-    match r with
-      | RvLval ?l =>
-        reify_lvalue isConst l types funcs uvars vars ltac:(fun uvars funcs l =>
-          let l := constr:(@SymRvLval types l) in k uvars funcs l)
-      | RvImm ?i =>
-        reify_expr isConst i types funcs uvars vars ltac:(fun uvars funcs i =>
-          let l := constr:(@SymRvImm types i) in k uvars funcs l)
-      | RvLabel ?l => 
-        let r := constr:(@SymRvLabel types l) in k uvars funcs r
-    end.
+Ltac reify_rvalue isConst r types funcs uvars vars k :=
+  match r with
+    | RvLval ?l =>
+      reify_lvalue isConst l types funcs uvars vars ltac:(fun uvars funcs l =>
+        let l := constr:(@SymRvLval types l) in k uvars funcs l)
+    | RvImm ?i =>
+      reify_expr isConst i types funcs uvars vars ltac:(fun uvars funcs i =>
+        let l := constr:(@SymRvImm types i) in k uvars funcs l)
+    | RvLabel ?l => 
+      let r := constr:(@SymRvLabel types l) in k uvars funcs r
+  end.
 
-  Ltac collectTypes_instr isConst i Ts :=
-    match i with
-      | Assign ?l ?r =>
-        let Ts := collectTypes_lvalue isConst l Ts in
+Ltac collectTypes_instr isConst i Ts :=
+  match i with
+    | Assign ?l ?r =>
+      let Ts := collectTypes_lvalue isConst l Ts in
         collectTypes_rvalue isConst r Ts
-      | Binop ?l ?r1 _ ?r2 =>
-        let Ts := collectTypes_lvalue isConst l Ts in
+    | Binop ?l ?r1 _ ?r2 =>
+      let Ts := collectTypes_lvalue isConst l Ts in
         let Ts := collectTypes_rvalue isConst r1 Ts in
-        collectTypes_rvalue isConst r2 Ts
-    end.
-  Ltac reify_instr isConst i types funcs uvars vars k :=
-    match i with
-      | Assign ?l ?r =>
-        reify_lvalue isConst l types funcs uvars vars ltac:(fun uvars funcs l =>
+          collectTypes_rvalue isConst r2 Ts
+  end.
+Ltac reify_instr isConst i types funcs uvars vars k :=
+  match i with
+    | Assign ?l ?r =>
+      reify_lvalue isConst l types funcs uvars vars ltac:(fun uvars funcs l =>
         reify_rvalue isConst r types funcs uvars vars ltac:(fun uvars funcs r =>
           let res := constr:(@SymAssign types l r) in k uvars funcs res))
-      | Binop ?l ?r1 ?o ?r2 =>
-        reify_lvalue isConst l types funcs uvars vars ltac:(fun uvars funcs l =>
+    | Binop ?l ?r1 ?o ?r2 =>
+      reify_lvalue isConst l types funcs uvars vars ltac:(fun uvars funcs l =>
         reify_rvalue isConst r1 types funcs uvars vars ltac:(fun uvars funcs r1 =>
-        reify_rvalue isConst r2 types funcs uvars vars ltac:(fun uvars funcs r2 =>
-          let res := constr:(@SymBinop types l r1 o r2) in k uvars funcs res)))
-    end.
+          reify_rvalue isConst r2 types funcs uvars vars ltac:(fun uvars funcs r2 =>
+            let res := constr:(@SymBinop types l r1 o r2) in k uvars funcs res)))
+  end.
 
-  Ltac collectTypes_instrs isConst is Ts :=
-    match is with
-      | nil => Ts
-      | ?i :: ?is => 
-        let Ts := collectTypes_instr isConst i Ts in
+Ltac collectTypes_instrs isConst is Ts :=
+  match is with
+    | nil => Ts
+    | ?i :: ?is => 
+      let Ts := collectTypes_instr isConst i Ts in
         collectTypes_instrs isConst is Ts
-    end.
-  Ltac reify_instrs isConst is types funcs uvars vars k :=
-    match is with
-      | nil => 
-        let is := constr:(@nil (sym_instr types)) in k uvars funcs is
-      | ?i :: ?is =>
-        reify_instr isConst i types funcs uvars vars ltac:(fun uvars funcs i =>
+  end.
+Ltac reify_instrs isConst is types funcs uvars vars k :=
+  match is with
+    | nil => 
+      let is := constr:(@nil (sym_instr types)) in k uvars funcs is
+    | ?i :: ?is =>
+      reify_instr isConst i types funcs uvars vars ltac:(fun uvars funcs i =>
         reify_instrs isConst is types funcs uvars vars ltac:(fun uvars funcs is =>
           let res := constr:(i :: is) in k uvars funcs res))
-    end.
+  end.
 
-  Ltac isConst e :=
-    match e with
-      | 0 => true
-      | S ?e => isConst e
-      | true => true
-      | false => true
-      | _ => false
-    end.
+Ltac isConst e :=
+  match e with
+    | 0 => true
+    | S ?e => isConst e
+    | true => true
+    | false => true
+    | _ => false
+  end.
 
-  Ltac find_reg st r :=
-    match goal with
-      | [ H : Regs st r = ?x |- _ ] => x
-      | _ => constr:((Regs st r, @refl_equal (option W) (Some (Regs st r))))
-    end.
+Ltac find_reg st r :=
+  match goal with
+    | [ H : Regs st r = ?x |- _ ] => x
+    | _ => constr:((Regs st r, @refl_equal (option W) (Some (Regs st r))))
+  end.
 
-  Ltac open_stateD H0 :=
-    cbv beta iota zeta delta 
-      [ stateD Expr.exprD Expr.applyD
-        EquivDec.equiv_dec 
-        Expr.Range Expr.Domain Expr.Denotation
-        Expr.EqDec_tvar Expr.tvar_rec Expr.tvar_rect
-        sumbool_rec sumbool_rect
-        Peano_dec.eq_nat_dec nat_rec nat_rect eq_rec_r eq_rec eq_rect eq_sym
-        nth_error map value
-        f_equal
+Ltac open_stateD H0 :=
+  cbv beta iota zeta delta 
+    [ stateD Expr.exprD Expr.applyD
+      EquivDec.equiv_dec 
+      Expr.Range Expr.Domain Expr.Denotation
+      Expr.EqDec_tvar Expr.tvar_rec Expr.tvar_rect
+      sumbool_rec sumbool_rect
+      Peano_dec.eq_nat_dec nat_rec nat_rect eq_rec_r eq_rec eq_rect eq_sym
+      nth_error map value
+      f_equal
 
-        Expr.AllProvable Expr.Provable Expr.tvarD types comparator
-      ] in H0; 
-      let a := fresh in 
-      let b := fresh in
-      let zz := fresh in destruct H0 as [ a [ b zz ] ] ;
-      destruct a as [ ? [ ? ? ] ];
-      repeat match type of zz with
-               | True => clear zz
-               | _ /\ _ => let v := fresh in destruct zz as [ v zz ]
-             end.
+      Expr.AllProvable Expr.Provable Expr.tvarD comparator
+    ] in H0; 
+    let a := fresh in 
+    let b := fresh in
+    let zz := fresh in destruct H0 as [ a [ b zz ] ] ;
+    destruct a as [ ? [ ? ? ] ];
+    repeat match type of zz with
+             | True => clear zz
+             | _ /\ _ => let v := fresh in destruct zz as [ v zz ]
+           end.
 
-  Ltac get_instrs st :=
-    let rec find_exact H Hs :=
-      match Hs with
-        | tt => false
-        | H :: _ => true
-        | _ :: ?Hs => find_exact H Hs
-      end
+Ltac get_instrs st :=
+  let rec find_exact H Hs :=
+    match Hs with
+      | tt => false
+      | H :: _ => true
+      | _ :: ?Hs => find_exact H Hs
+    end
     in
     let rec get_instrs st ignore :=
       match goal with
@@ -939,7 +886,7 @@ Module BedrockEvaluator.
           match find_exact H ignore with
             | false =>
               let v := get_instrs st (H, ignore) in
-              constr:((((l,r), H), v))
+                constr:((((l,r), H), v))
           end
         | [ H : Structured.evalCond ?l _ ?r _ st = None |- _ ] =>
           constr:((((l,r), H), tt))
@@ -950,260 +897,260 @@ Module BedrockEvaluator.
           constr:(((is, H), tt))
         | [ |- _ ] => tt
       end
-    in get_instrs st tt.
-  Ltac collectAllTypes_instrs is Ts :=
-    match is with
-      | tt => Ts
-      | (((?l,?r), _), ?is) =>
-        let Ts := collectTypes_rvalue ltac:(isConst) l Ts in
+      in get_instrs st tt.
+Ltac collectAllTypes_instrs is Ts :=
+  match is with
+    | tt => Ts
+    | (((?l,?r), _), ?is) =>
+      let Ts := collectTypes_rvalue ltac:(isConst) l Ts in
         let Ts := collectTypes_rvalue ltac:(isConst) r Ts in
+          collectAllTypes_instrs is Ts
+    | ((?i, _), ?is) =>
+      let Ts := collectTypes_instrs ltac:(isConst) i Ts in
         collectAllTypes_instrs is Ts
-      | ((?i, _), ?is) =>
-        let Ts := collectTypes_instrs ltac:(isConst) i Ts in
-        collectAllTypes_instrs is Ts
-    end.
+  end.
 
-  Ltac build_path types instrs st uvars vars funcs k :=
-    match instrs with
-      | tt => 
-        let is := constr:(nil : @istream types) in
-        let pf := constr:(refl_equal (Some st)) in
-        k uvars funcs is (Some st) pf
-      | ((?i, ?H), ?is) =>
-        match type of H with
-          | Structured.evalCond ?l ?t ?r _ ?st = ?st' =>
-            reify_rvalue ltac:(isConst) l types funcs uvars vars ltac:(fun uvars funcs l =>
-              reify_rvalue ltac:(isConst) r types funcs uvars vars ltac:(fun uvars funcs r =>
-                match st' with
-                  | None => 
-                    let i := constr:(inr (@SymAssertCond types l t r st') :: (nil : @istream types)) in
-                    k uvars funcs i (@None state) H
-                  | Some ?st'' => 
-                    build_path types is st uvars vars funcs ltac:(fun uvars funcs is sf pf =>
-                      let i := constr:(inr (@SymAssertCond types l t r st') :: is) in
-                      let pf := constr:(@conj _ _ H pf) in
-                      k uvars funcs i sf pf)
-                end))
-          | evalInstrs _ ?st _ = ?st' =>
-            reify_instrs ltac:(isConst) i types funcs uvars vars ltac:(fun uvars funcs sis =>
+Ltac build_path types instrs st uvars vars funcs k :=
+  match instrs with
+    | tt => 
+      let is := constr:(nil : @istream types) in
+      let pf := constr:(refl_equal (Some st)) in
+      k uvars funcs is (Some st) pf
+    | ((?i, ?H), ?is) =>
+      match type of H with
+        | Structured.evalCond ?l ?t ?r _ ?st = ?st' =>
+          reify_rvalue ltac:(isConst) l types funcs uvars vars ltac:(fun uvars funcs l =>
+            reify_rvalue ltac:(isConst) r types funcs uvars vars ltac:(fun uvars funcs r =>
               match st' with
                 | None => 
-                  let i := constr:(inl (sis, None) :: (nil : @istream types)) in
+                  let i := constr:(inr (@SymAssertCond types l t r st') :: (nil : @istream types)) in
                   k uvars funcs i (@None state) H
-                | Some ?st'' =>
-                  build_path types is st'' uvars vars funcs ltac:(fun uvars funcs is sf pf =>
-                    let i := constr:(inl (sis, st') :: is) in
+                | Some ?st'' => 
+                  build_path types is st uvars vars funcs ltac:(fun uvars funcs is sf pf =>
+                    let i := constr:(inr (@SymAssertCond types l t r st') :: is) in
                     let pf := constr:(@conj _ _ H pf) in
                     k uvars funcs i sf pf)
-              end)
-        end
-    end.              
+              end))
+        | evalInstrs _ ?st _ = ?st' =>
+          reify_instrs ltac:(isConst) i types funcs uvars vars ltac:(fun uvars funcs sis =>
+            match st' with
+              | None => 
+                let i := constr:(inl (sis, None) :: (nil : @istream types)) in
+                  k uvars funcs i (@None state) H
+              | Some ?st'' =>
+                build_path types is st'' uvars vars funcs ltac:(fun uvars funcs is sf pf =>
+                  let i := constr:(inl (sis, st') :: is) in
+                  let pf := constr:(@conj _ _ H pf) in
+                  k uvars funcs i sf pf)
+            end)
+      end
+  end.
 
-  Goal forall (cs : codeSpec W (settings * state)) (stn : settings) st st',
-      Structured.evalCond (RvImm (natToW 0)) IL.Eq (RvImm (natToW 0)) stn st' = Some true ->
-      evalInstrs stn st (Assign Rp (RvImm (natToW 0)) :: nil) = Some st' -> 
-      True.
-    intros.
+Goal forall (cs : codeSpec W (settings * state)) (stn : settings) st st',
+  Structured.evalCond (RvImm (natToW 0)) IL.Eq (RvImm (natToW 0)) stn st' = Some true ->
+  evalInstrs stn st (Assign Rp (RvImm (natToW 0)) :: nil) = Some st' -> 
+  True.
+  intros.
+  match goal with
+    | [ |- _ ] => 
+      let i := get_instrs st in
+      let Ts := constr:(@nil Type) in
+      let Ts := collectAllTypes_instrs i Ts in
+      let types_ := eval unfold bedrock_types in bedrock_types in
+      let types_ := Expr.extend_all_types Ts types_ in
+      let typesV := fresh "types" in
+      pose (typesV := types_) ;
+      let v := constr:(nil : env typesV) in
+      let f := constr:(nil : functions typesV) in
+      build_path typesV i st v v f ltac:(fun uvars funcs is sf pf =>
+        assert (@istreamD typesV funcs uvars v is stn st sf) by (exact pf))
+  end.
+Abort.
+
+(** TODO:
+ ** - To avoid reflecting for each basic block, I need to gather all the
+ **   hypotheses and information that will go into the term at the beginning
+ ** - The "algorithm" is:
+ **   1) reflect everything!
+ **   2) forward unfolding
+ **   3) symbolic evaluation
+ **   4) backward unfolding
+ **   5) cancelation
+ ** - steps 2-4 are repeated for each basic block that we evaluate
+ ** NOTE:
+ ** - [isConst] is an ltac function of type [* -> bool]
+ ** - [prover] is an ltac with "type" (assuming [PR] is the prover to use)
+ **     [forall ts (fs : functions ts), ProverT_correct ts PR fs]. 
+ ** - [plugin] is an ltac with "type" (assuming [PL] is the plugin to use)
+ **     [forall ts pcT stT (fs : functions ts) (ps : sfunctions ts pcT stT), SymEvaluator_correct ts fs ps PL]
+ ** - [unfolder] is an ltac with "type" (assuming [U] is the unfolder to use)
+ **     [forall ts pcT stT (fs : functions ts) (ps : sfunctions ts pcT stT), LearnHook_correct ts (Facts PR) U fs ps]
+ ** - [simplifier] is an ltac that takes a hypothesis names and simplifies it
+ **     (this should be implmented using [cbv beta iota zeta delta [ ... ] in H])
+ **     (it is recommended/necessary to call [sym_evaluator] or import its simplification)
+ ** - [Ts] is the list of seed types, [list type]
+ ** - [Fs] is an ltac that produces the list of seed functions, [tuple-of (_ -> ... -> _)]
+ **     (values that are [tt] may be overridden)
+ ** - [SFs] is an ltac that produces the list of seed predicates, [tuple-of (_ -> ... -> _ -> hprop _)]
+ **     (values that are [tt] may be overriden)
+ **)
+Ltac sym_eval isConst prover plugin unfolder simplifier Ts Fs SFs :=
+  let rec init_from st :=
     match goal with
-      | [ |- _ ] => 
-        let i := get_instrs st in
-        let Ts := constr:(@nil Type) in
-        let Ts := collectAllTypes_instrs i Ts in
-        let types_ := eval unfold bedrock_types in bedrock_types in
-        let types_ := Expr.extend_all_types Ts types_ in
-        let typesV := fresh "types" in
-        pose (typesV := types_) ;
-        let v := constr:(nil : env typesV) in
-        let f := constr:(nil : functions typesV) in
-        build_path typesV i st v v f ltac:(fun uvars funcs is sf pf =>
-          assert (@istreamD typesV funcs uvars v is stn st sf) by (exact pf))
-    end.
-  Abort.
+      | [ H : evalInstrs _ ?st' _ = Some st |- _ ] => init_from st'
+      | [ |- _ ] => st
+    end
+  in          
+  let shouldReflect P :=
+    match P with
+      | evalInstrs _ _ _ = _ => false
+      | Structured.evalCond _ _ _ _ _ = _ => false
+      | @PropX.interp _ _ _ _ => false
+      | @PropX.valid _ _ _ _ _ => false
+      | @eq ?X _ _ => 
+        match X with
+          | context [ PropX.PropX ] => false
+          | context [ PropX.spec ] => false
+        end
+      | forall x, _ => false
+      | exists x, _ => false
+      | _ => true
+    end
+  in
+  let Ts := 
+    match Ts with
+      | tt => constr:(@nil Type)
+      | _ => match type of Ts with
+               | list Type => Ts
+               | ?TTs => fail 10 "Ts must have type (list Type), got " TTs
+             end
+    end
+  in
+  match Fs with 
+    | tt => idtac
+    | (_ , _) => idtac 
+    | _ => fail 10 "Fs must be a tuple of functions, got " Fs
+  end ;
+  match SFs with 
+    | tt => idtac
+    | (_ , _) => idtac 
+    | _ => fail 10 "SFs must be a tuple of predicates, got " Fs
+  end ;
+  let stn_st_SF :=
+    match goal with
+      | [ H : interp _ (![ ?SF ] ?X) |- _ ] => constr:((X, (SF, H)))
+      | [ H : Structured.evalCond _ _ _ ?stn ?st = _ |- _ ] => 
+        let st := init_from st in
+        constr:(((stn, st), tt))
+      | [ H : IL.evalInstrs ?stn ?st _ = _ |- _ ] =>
+        let st := init_from st in
+        constr:(((stn, st), tt))
+      | [ |- _ ] => tt
+    end
+  in
+  let cs :=
+    match goal with
+      | [ H : codeSpec _ _ |- _ ] => H
+    end
+  in
+  match stn_st_SF with
+    | tt =>
+      idtac "couldn't find anything to symbolically evaluate!" 
+    | ((?stn, ?st), ?SF) =>
+      match find_reg st Rp with
+        | (?rp_v, ?rp_pf) =>
+          match find_reg st Sp with
+            | (?sp_v, ?sp_pf) =>
+              match find_reg st Rv with
+                | (?rv_v, ?rv_pf) =>
+                  let all_instrs := get_instrs st in
+                  let all_props := Expr.collect_props shouldReflect in
+                  let pures := Expr.props_types all_props in
 
-  (** TODO:
-   ** - To avoid reflecting for each basic block, I need to gather all the
-   **   hypotheses and information that will go into the term at the beginning
-   ** - The "algorithm" is:
-   **   1) reflect everything!
-   **   2) forward unfolding
-   **   3) symbolic evaluation
-   **   4) backward unfolding
-   **   5) cancelation
-   ** - steps 2-4 are repeated for each basic block that we evaluate
-   ** NOTE:
-   ** - [isConst] is an ltac function of type [* -> bool]
-   ** - [prover] is an ltac with "type" (assuming [PR] is the prover to use)
-   **     [forall ts (fs : functions ts), ProverT_correct ts PR fs]. 
-   ** - [plugin] is an ltac with "type" (assuming [PL] is the plugin to use)
-   **     [forall ts pcT stT (fs : functions ts) (ps : sfunctions ts pcT stT), SymEvaluator_correct ts fs ps PL]
-   ** - [unfolder] is an ltac with "type" (assuming [U] is the unfolder to use)
-   **     [forall ts pcT stT (fs : functions ts) (ps : sfunctions ts pcT stT), LearnHook_correct ts (Facts PR) U fs ps]
-   ** - [simplifier] is an ltac that takes a hypothesis names and simplifies it
-   **     (this should be implmented using [cbv beta iota zeta delta [ ... ] in H])
-   **     (it is recommended/necessary to call [sym_evaluator] or import its simplification)
-   ** - [Ts] is the list of seed types, [list type]
-   ** - [Fs] is an ltac that produces the list of seed functions, [tuple-of (_ -> ... -> _)]
-   **     (values that are [tt] may be overridden)
-   ** - [SFs] is an ltac that produces the list of seed predicates, [tuple-of (_ -> ... -> _ -> hprop _)]
-   **     (values that are [tt] may be overriden)
-   **)
-  Ltac sym_eval isConst prover plugin unfolder simplifier Ts Fs SFs :=
-    let rec init_from st :=
-      match goal with
-        | [ H : evalInstrs _ ?st' _ = Some st |- _ ] => init_from st'
-        | [ |- _ ] => st
-      end
-    in          
-    let shouldReflect P :=
-      match P with
-        | evalInstrs _ _ _ = _ => false
-        | Structured.evalCond _ _ _ _ _ = _ => false
-        | @PropX.interp _ _ _ _ => false
-        | @PropX.valid _ _ _ _ _ => false
-        | @eq ?X _ _ => 
-          match X with
-            | context [ PropX.PropX ] => false
-            | context [ PropX.spec ] => false
-          end
-        | forall x, _ => false
-        | exists x, _ => false
-        | _ => true
-      end
-    in
-    let Ts := 
-      match Ts with
-        | tt => constr:(@nil Type)
-        | _ => match type of Ts with
-                 | list Type => Ts
-                 | ?TTs => fail 10 "Ts must have type (list Type), got " TTs
-               end
-      end
-    in
-    match Fs with 
-      | tt => idtac
-      | (_ , _) => idtac 
-      | _ => fail 10 "Fs must be a tuple of functions, got " Fs
-    end ;
-    match SFs with 
-      | tt => idtac
-      | (_ , _) => idtac 
-      | _ => fail 10 "SFs must be a tuple of predicates, got " Fs
-    end ;
-    let stn_st_SF :=
-      match goal with
-        | [ H : interp _ (![ ?SF ] ?X) |- _ ] => constr:((X, (SF, H)))
-        | [ H : Structured.evalCond _ _ _ ?stn ?st = _ |- _ ] => 
-          let st := init_from st in
-          constr:(((stn, st), tt))
-        | [ H : IL.evalInstrs ?stn ?st _ = _ |- _ ] =>
-          let st := init_from st in
-          constr:(((stn, st), tt))
-        | [ |- _ ] => tt
-      end
-    in
-    let cs :=
-      match goal with
-        | [ H : codeSpec _ _ |- _ ] => H
-      end
-    in
-    match stn_st_SF with
-      | tt =>
-        idtac "couldn't find anything to symbolically evaluate!" 
-      | ((?stn, ?st), ?SF) =>
-        match find_reg st Rp with
-          | (?rp_v, ?rp_pf) =>
-            match find_reg st Sp with
-              | (?sp_v, ?sp_pf) =>
-                match find_reg st Rv with
-                  | (?rv_v, ?rv_pf) =>
-                    let all_instrs := get_instrs st in
-                    let all_props := Expr.collect_props shouldReflect in
-                    let pures := Expr.props_types all_props in
-
-                    let regs := constr:((rp_v, (sp_v, (rv_v, tt)))) in
-                    (** collect the raw types **)
-                    let Ts := collectAllTypes_instrs all_instrs Ts in
-                    let Ts := Expr.collectTypes_exprs ltac:(isConst) regs Ts in
-                    let Ts := Expr.collectTypes_exprs ltac:(isConst) pures Ts in
-                    let Ts := 
-                      match SF with
-                        | tt => Ts 
-                        | (?SF, _) => SEP.collectAllTypes_sexpr isConst Ts (SF :: nil)
-                      end
-                    in
-                    let Ts := Expr.collectAllTypes_funcs Ts Fs in
-                    let Ts := SEP.collectAllTypes_sfuncs Ts SFs in
-                    (** check for potential universe problems **)
-                    match Ts with
-                      | context [ PropX.PropX ] => 
-                        fail 1000 "found PropX in types list"
-                          "(this causes universe inconsistencies)"
-                      | context [ PropX.spec ] => 
-                        fail 1000 "found PropX in types list"
-                          "(this causes universe inconsistencies)"
-                      | _ => idtac
-                    end;
-                    (** elaborate the types **)
-                    let types_ := eval unfold bedrock_types in bedrock_types in
-                    let types_ := Expr.extend_all_types Ts types_ in
-                    let typesV := fresh "types" in
-                    pose (typesV := types_);
-                    (** **)
-                    let pcT := constr:(tvType 0) in
-                    let stT := constr:(tvType 1) in
-                    (** build the variables **)
-                    let uvars := eval simpl in (@nil _ : Expr.env typesV) in
-                    let vars := uvars in
-                    (** build the base functions **)
-                    let funcs := eval unfold bedrock_funcs in (@bedrock_funcs typesV) in
-                    let funcs := Expr.getAllFunctions typesV funcs Fs in
-                    let funcs := eval simpl in funcs in
-                    (** build the base sfunctions **)
-                    let sfuncs := constr:(@nil (@SEP.ssignature typesV pcT stT)) in
-                    let sfuncs := SEP.getAllSFunctions pcT stT typesV sfuncs SFs in
-                    (** reflect the expressions **)
-                    Expr.reify_exprs ltac:(isConst) pures typesV funcs uvars vars ltac:(fun uvars funcs pures =>
-                    let proofs := Expr.props_proof all_props in
-                    Expr.reify_expr ltac:(isConst) rp_v typesV funcs uvars vars ltac:(fun uvars funcs rp_v =>
-                    Expr.reify_expr ltac:(isConst) sp_v typesV funcs uvars vars ltac:(fun uvars funcs sp_v =>
-                    Expr.reify_expr ltac:(isConst) rv_v typesV funcs uvars vars ltac:(fun uvars funcs rv_v =>
-                      let finish H syms :=
-                        let rec unfold_all syms :=
-                          match syms with
-                            | tt => idtac
-                            | (?X, ?Y) => subst X ; unfold_all Y
-                            | ?X => subst X
-                          end
-                        in
-                        unfold_all syms ; 
-                        first [ simplifier H | fail 100000 "simplifier failed!" ] ;
-                        (try assumption || destruct H as [ [ ? [ ? ? ] ] [ ? ? ] ])
+                  let regs := constr:((rp_v, (sp_v, (rv_v, tt)))) in
+                  (** collect the raw types **)
+                  let Ts := collectAllTypes_instrs all_instrs Ts in
+                  let Ts := Expr.collectTypes_exprs ltac:(isConst) regs Ts in
+                  let Ts := Expr.collectTypes_exprs ltac:(isConst) pures Ts in
+                  let Ts := 
+                    match SF with
+                      | tt => Ts 
+                      | (?SF, _) => SEP.collectAllTypes_sexpr isConst Ts (SF :: nil)
+                    end
+                  in
+                  let Ts := Expr.collectAllTypes_funcs Ts Fs in
+                  let Ts := SEP.collectAllTypes_sfuncs Ts SFs in
+                  (** check for potential universe problems **)
+                  match Ts with
+                    | context [ PropX.PropX ] => 
+                      fail 1000 "found PropX in types list"
+                        "(this causes universe inconsistencies)"
+                    | context [ PropX.spec ] => 
+                      fail 1000 "found PropX in types list"
+                        "(this causes universe inconsistencies)"
+                    | _ => idtac
+                  end;
+                  (** elaborate the types **)
+                  let types_ := eval unfold bedrock_types in bedrock_types in
+                  let types_ := Expr.extend_all_types Ts types_ in
+                  let typesV := fresh "types" in
+                  pose (typesV := types_);
+                  (** **)
+                  let pcT := constr:(tvType 0) in
+                  let stT := constr:(tvType 1) in
+                  (** build the variables **)
+                  let uvars := eval simpl in (@nil _ : Expr.env typesV) in
+                  let vars := uvars in
+                  (** build the base functions **)
+                  let funcs := eval unfold bedrock_funcs in (@bedrock_funcs typesV) in
+                  let funcs := Expr.getAllFunctions typesV funcs Fs in
+                  let funcs := eval simpl in funcs in
+                  (** build the base sfunctions **)
+                  let sfuncs := constr:(@nil (@SEP.ssignature typesV pcT stT)) in
+                  let sfuncs := SEP.getAllSFunctions pcT stT typesV sfuncs SFs in
+                  (** reflect the expressions **)
+                  Expr.reify_exprs ltac:(isConst) pures typesV funcs uvars vars ltac:(fun uvars funcs pures =>
+                  let proofs := Expr.props_proof all_props in
+                  Expr.reify_expr ltac:(isConst) rp_v typesV funcs uvars vars ltac:(fun uvars funcs rp_v =>
+                  Expr.reify_expr ltac:(isConst) sp_v typesV funcs uvars vars ltac:(fun uvars funcs sp_v =>
+                  Expr.reify_expr ltac:(isConst) rv_v typesV funcs uvars vars ltac:(fun uvars funcs rv_v =>
+                    let finish H syms :=
+                      let rec unfold_all syms :=
+                        match syms with
+                          | tt => idtac
+                          | (?X, ?Y) => unfold_all X ; unfold_all Y
+                          | ?X => subst X
+                        end
                       in
-                      build_path typesV all_instrs st uvars vars funcs ltac:(fun uvars funcs is fin_state is_pf =>
-                        match SF with
-                          | tt =>
-                            let funcsV := fresh "funcs" in
-                            pose (funcsV := funcs) ;
-                            let sfuncsV := fresh "sfuncs" in
-                            pose (sfuncsV := sfuncs) ;
-                            let proverCV := fresh "proverC" in
-                            let proverC := prover typesV funcsV in
-                            pose (proverCV := proverC) ;
-                            let pluginCV := fresh "plugin" in
-                            let pluginC := plugin typesV pcT stT funcsV sfuncsV in
-                            pose (pluginCV := pluginC) ;
-                            let unfolderC := unfolder typesV pcT stT funcsV sfuncsV in
-                            let unfolderCV := fresh "unfolder" in
-                            pose (unfolderCV := unfolderC) ;
-                            generalize (@stateD_proof_no_heap typesV funcsV _ proverCV
-                              uvars vars sfuncsV st sp_v rv_v rp_v 
-                              sp_pf rv_pf rp_pf pures proofs cs stn) ;
-                            let H_stateD := fresh in
-                            intro H_stateD ;
-                            (apply (@sym_eval_any typesV funcsV sfuncsV _ pluginCV _ proverCV _ unfolderCV
-                                stn uvars vars fin_state st is is_pf) in H_stateD ;
-                             let syms := constr:((typesV, (funcsV, (sfuncsV, (proverCV, (pluginCV, unfolderCV)))))) in
-                             finish H_stateD syms) || fail 100000 "couldn't apply sym_eval_any! (SF case)"
+                      unfold_all syms ; 
+                      first [ simplifier H | fail 100000 "simplifier failed!" ] ;
+                      (try assumption || destruct H as [ [ ? [ ? ? ] ] [ ? ? ] ])
+                    in
+                    build_path typesV all_instrs st uvars vars funcs ltac:(fun uvars funcs is fin_state is_pf =>
+                      match SF with
+                        | tt =>
+                          let funcsV := fresh "funcs" in
+                          pose (funcsV := funcs) ;
+                          let sfuncsV := fresh "sfuncs" in
+                          pose (sfuncsV := sfuncs) ;
+                          let proverCV := fresh "proverC" in
+                          let proverC := prover typesV funcsV in
+                          pose (proverCV := proverC) ;
+                          plugin typesV pcT stT funcsV sfuncsV ltac:(fun plugin_syms pluginC =>
+                          let pluginCV := fresh "plugin" in
+                          pose (pluginCV := pluginC) ;
+                          let unfolderC := unfolder typesV pcT stT funcsV sfuncsV in
+                          let unfolderCV := fresh "unfolder" in
+                          pose (unfolderCV := unfolderC) ;
+                          generalize (@stateD_proof_no_heap typesV funcsV _ proverCV
+                            uvars vars sfuncsV st sp_v rv_v rp_v 
+                            sp_pf rv_pf rp_pf pures proofs cs stn) ;
+                          let H_stateD := fresh in
+                          intro H_stateD ;
+                          (apply (@sym_eval_any typesV funcsV sfuncsV _ pluginCV _ proverCV _ unfolderCV
+                              stn uvars vars fin_state st is is_pf) in H_stateD ;
+                           let syms := constr:((typesV, (funcsV, (sfuncsV, (proverCV, (pluginCV, unfolderCV)))))) in
+                           finish H_stateD syms) || fail 100000 "couldn't apply sym_eval_any! (non-SF case)"
 (*
                              first [
                                generalize (@sym_eval_any typesV funcsV sfuncsV _ pluginCV _ proverCV stn uvars vars _ _ _ path) |
@@ -1215,10 +1162,10 @@ Module BedrockEvaluator.
                                generalize (@sym_eval_any typesV funcsV sfuncsV) |
                                generalize (@sym_eval_any typesV funcsV) |
                                generalize (@sym_eval_any typesV)
-                             ] *)
+                             ] *))
                         | (?SF, ?H_interp) =>
                           SEP.reify_sexpr ltac:(isConst) SF typesV funcs pcT stT sfuncs uvars vars 
-                          ltac:(fun uvars funcs sfuncs SF => 
+                          ltac:(fun uvars funcs sfuncs SF =>
                             let funcsV := fresh "funcs" in
                             pose (funcsV := funcs) ;
                             let sfuncsV := fresh "sfuncs" in
@@ -1226,7 +1173,7 @@ Module BedrockEvaluator.
                             let proverC := prover typesV funcsV in
                             let proverCV := fresh "proverC" in
                             pose (proverCV := proverC) ;
-                            let pluginC := plugin typesV pcT stT funcsV sfuncsV in
+                            plugin typesV pcT stT funcsV sfuncsV ltac:(fun plugin_syms pluginC =>
                             let pluginCV := fresh "plugin" in
                             pose (pluginCV := pluginC) ;
                             let unfolderC := unfolder typesV pcT stT funcsV sfuncsV in
@@ -1237,13 +1184,13 @@ Module BedrockEvaluator.
                               sp_pf rv_pf rp_pf pures proofs SF _ (refl_equal _)) in H_interp ;
                             (apply (@sym_eval_any typesV funcsV sfuncsV _ pluginCV _ proverCV _ unfolderCV
                               stn uvars vars fin_state st is is_pf) in H_interp ;
-                             let syms := constr:((typesV, (funcsV, (sfuncsV, (proverCV, (pluginCV, unfolderCV)))))) in
-                             finish H_interp syms) || fail 100000 "couldn't apply sym_eval_any! (SF case)" (* ||
+                             let syms := constr:((plugin_syms, (typesV, (funcsV, (sfuncsV, (proverCV, (pluginCV, unfolderCV))))))) in
+                             finish H_interp syms) || (*fail 100000 "couldn't apply sym_eval_any! (SF case)" || *)
                             first [ 
                               generalize (@sym_eval_any typesV funcsV sfuncsV _ pluginCV _ proverCV _ unfolderCV
                                 stn uvars vars fin_state st is is_pf) ; idtac "A" |
                               pose is_pf ; generalize (@sym_eval_any typesV funcsV sfuncsV _ pluginCV _ proverCV _ unfolderCV
-                                stn uvars vars fin_state st is) ; idtac "B" (*|
+                                stn uvars vars fin_state st is) ; idtac "B" |
                                 generalize (@sym_eval_any typesV funcsV sfuncsV _ pluginCV _ proverCV _ unfolderCV
                                   stn uvars) ; idtac "C" |
                                 generalize (@sym_eval_any typesV funcsV sfuncsV _ pluginCV _ proverCV _ unfolderCV
@@ -1251,268 +1198,199 @@ Module BedrockEvaluator.
                                 generalize (@sym_eval_any typesV funcsV sfuncsV _ pluginCV _ proverCV _ unfolderCV) ; idtac "E" |
                                 generalize (@sym_eval_any typesV funcsV sfuncsV _ pluginCV _ proverCV) ; idtac "F" |
                                 generalize (@sym_eval_any typesV funcsV sfuncsV _ pluginCV) ; idtac "G" |
-                                generalize (@sym_eval_any typesV funcsV sfuncsV) ; idtac "H" *) ] *)
-                            )
+                                generalize (@sym_eval_any typesV funcsV sfuncsV) ; idtac "H" ] 
+                            ))
                       end)))))
-                end
+              end
+          end
+      end
+  end.
+
+Ltac sym_evaluator H := 
+  cbv beta iota zeta delta
+    [ sym_evalInstrs sym_evalInstr sym_evalLval sym_evalRval sym_evalLoc sym_evalStream sym_assertTest
+      sym_setReg sym_getReg
+      SepExpr.pures SepExpr.impures SepExpr.other
+      SymMem SymRegs SymPures SymVars SymUVars
+      SEP.star_SHeap SEP.liftSHeap SEP.multimap_join 
+      Expr.SemiDec_expr Expr.expr_seq_dec Expr.tvar_val_sdec Expr.Eq Expr.liftExpr
+      app map nth_error value error fold_right hd hd_error tl tail rev
+      Decidables.seq_dec 
+      DepList.hlist_hd DepList.hlist_tl 
+      SepExpr.FM.find SepExpr.FM.add SepExpr.FM.remove SepExpr.FM.map SepExpr.FM.empty SepExpr.FM.fold
+      Compare_dec.lt_eq_lt_dec nat_rec nat_rect Peano_dec.eq_nat_dec sumbool_rec sumbool_rect
+      EquivDec.equiv_dec EquivDec.nat_eq_eqdec
+      f_equal 
+      bedrock_funcs_r bedrock_types
+      fst snd
+      Env.repr Env.updateAt SEP.substV
+
+      stateD Expr.exprD 
+      Expr.applyD Expr.exprD Expr.Range Expr.Domain Expr.Denotation Expr.lookupAs
+      Expr.AllProvable Expr.Provable Expr.tvarD
+      SEP.sheapD SEP.starred SEP.sexprD
+      EquivDec.equiv_dec Expr.EqDec_tvar Expr.tvar_rec Expr.tvar_rect 
+      Logic.eq_sym eq_sym f_equal
+      eq_rec_r eq_rect eq_rec
+      nat_rec nat_rect
+      sumbool_rec sumbool_rect
+      
+      SEP.himp SEP.sexprD Expr.Impl 
+      Expr.applyD Expr.exprD Expr.Range Expr.Domain Expr.Denotation 
+      Expr.lookupAs
+      SepExpr.SDenotation SepExpr.SDomain
+      EquivDec.nat_eq_eqdec  
+      SEP.sheapD SEP.sepCancel
+      SepExpr.impures SepExpr.pures SepExpr.other
+      SEP.star_SHeap SEP.unify_remove_all 
+      SEP.multimap_join SEP.liftSHeap SEP.unify_remove SEP.starred 
+      Expr.tvarD Expr.Eq
+      
+      SepExpr.FM.fold SepExpr.FM.find SepExpr.FM.add SepExpr.FM.empty 
+      bedrock_types 
+        
+      Compare_dec.lt_eq_lt_dec Peano_dec.eq_nat_dec
+      SepExpr.FM.map ExprUnify.exprUnifyArgs ExprUnify.empty_Subst
+      ExprUnify.exprUnify ExprUnify.fold_left_2_opt 
+      EquivDec.equiv_dec Expr.EqDec_tvar Expr.tvar_rec Expr.tvar_rect 
+      ExprUnify.get_Eq
+      orb
+        
+      Expr.typeof comparator
+
+      fPlus fMinus fMult
+      
+      repr_combine default footprint repr' updateAt Default_signature nil_Repr EmptySet_type SEP.Default_ssignature
+      bedrock_funcs_r bedrock_types_r
+
+      Summarize Learn Prove
+      
+      MEVAL.smemeval_read_word MEVAL.smemeval_write_word
+      
+      EquivDec_nat Peano_dec.eq_nat_dec
+
+      Prover.Prove Prover.Facts Prover.Learn Prover.Summarize
+    ] in H.
+
+Implicit Arguments istreamD [ types' ].
+
+Module Demo.
+  Require Provers.
+
+  Definition defaultLearnHook types : LearnHook types (tvType 0) (tvType 1) :=
+    fun _ x _ => x.
+
+  Theorem defaultLearnHook_correct types funcs preds 
+    : @LearnHook_correct (repr bedrock_types_r types) (@defaultLearnHook _) funcs preds.
+  Proof.
+    econstructor. unfold defaultLearnHook. intros; subst; auto.
+  Qed.
+
+  Ltac simplifier H :=
+    Provers.unfold_reflexivityProver H ;
+    MEVAL.Default.unfolder H ;
+    cbv delta [ 
+      defaultLearnHook
+    ] in H; sym_evaluator H.
+  
+  Definition demo_evaluator ts (fs : functions (repr bedrock_types_r ts)) ps := 
+    @MEVAL.Default.MemEvaluator_default_correct _ (tvType 0) (tvType 1) fs ps (settings * state) (tvType 0) (tvType 0) 
+    (@IL_mem_satisfies ts)
+    (@IL_ReadWord ts)
+    (@IL_WriteWord ts).
+
+  Goal forall (cs : codeSpec W (settings * state)) (stn : settings) st st' SF,
+    PropX.interp cs (SepIL.SepFormula.sepFormula SF (stn, st)) -> 
+    Structured.evalCond (RvImm (natToW 0)) IL.Eq (RvImm (natToW 0)) stn st' = Some true ->
+    evalInstrs stn st (Assign Rp (RvImm (natToW 0)) :: nil) = Some st' -> 
+    Regs st' Rp = natToW 0.
+  Proof.
+    intros.
+    Time sym_eval ltac:(isConst) 
+      ltac:(fun ts fs => constr:(@Provers.reflexivityProver_correct ts fs)) (* prover *)
+      ltac:(fun ts pc st fs ps k => let res := constr:(@demo_evaluator ts fs ps) in k tt res) (* memory evaluator *)
+      ltac:(fun ts pc st fs ps => constr:(@defaultLearnHook_correct ts fs ps)) (* unfolder *)
+      simplifier tt tt tt.
+    intuition; 
+    congruence.
+  Qed.
+End Demo.
+
+Module PluginEvaluator.
+  
+  Definition plugin_evaluator ts (fs : functions (repr bedrock_types_r ts)) ps evals consistent_pf := 
+    @MEVAL.Plugin.CompositeMemEvaluator_correct _ (tvType 0) (tvType 1) evals fs ps (settings * state) (tvType 0) (tvType 0)
+    (@IL_mem_satisfies ts)
+    (@IL_ReadWord ts)
+    (@IL_WriteWord ts)
+    consistent_pf.
+
+  (** This Ltac builds a function that can be instantiated to build a composite evaluator.
+   ** It should be applied to one argument and passed as the 3rd argument to [sym_eval].
+   ** Arguments:
+   ** - [known] is a tuple of [forall ts fs, @MemEvalPred_correct ts ? (tvType 0) (tvType 1) ? (tvType 0) (tvType 0) ... ]
+   **)
+  Ltac composite_eval known :=
+    let rec find_in p ls acc :=
+      match ls with
+        | nil => fail 100000 " didn't find " p
+        | ?l :: ?ls =>
+          match Reflect.unifies (SDenotation l) p with
+            | true => acc
+            | false => 
+              find_in p ls (S acc)
+          end
+      end
+    in
+    fun ts _pc _st fs ps k =>
+      let psVal := eval unfold ps in ps in
+      let rec build_pf known k :=
+        match known with
+          | tt => 
+            let r := constr:(@nil (nat * MEVAL.Plugin.MemEvalPred ts)) in
+            let pf := constr:(I) in
+            k r pf
+          | (?L, ?known) =>
+            let Z := type of L in
+            match type of L with
+              | forall ts,  forall fs, @MEVAL.Plugin.MemEvalPred_correct _ _ _ _ _ _ _ _ _ _ (@?s ts) _ =>
+                let p := eval simpl SDenotation in (SDenotation (s ts)) in
+                (** TODO: find [p] in [ps] **)
+                let idx := find_in p psVal 0 in                  
+
+                build_pf known ltac:(fun res pf =>
+                  let ZZZ := constr:(@L ts fs) in
+                  let E :=
+                    match type of ZZZ with
+                      | @MEVAL.Plugin.MemEvalPred_correct _ ?P _ _ _ _ _ _ _ _ _ _ => P
+                    end
+                  in
+                  let f := constr:((idx, E) :: res) in
+                  let pf := constr:(@conj _ _ ZZZ pf) in
+                  k f pf)              
             end
         end
-    end.
+      in 
+      build_pf known ltac:(fun evals consistent_pf =>
+        let evalsV := fresh "evals" in
+        pose (evalsV := evals) ;
+        let consistentV := fresh "consistent" in
+        let res := constr:(@plugin_evaluator ts fs ps evalsV consistent_pf) in
+        k evalsV res).
+  
+ Goal forall (cs : codeSpec W (settings * state)) (stn : settings) st st' SF,
+    PropX.interp cs (SepIL.SepFormula.sepFormula SF (stn, st)) -> 
+    Structured.evalCond (RvImm (natToW 0)) IL.Eq (RvImm (natToW 0)) stn st' = Some true ->
+    evalInstrs stn st (Assign Rp (RvImm (natToW 0)) :: nil) = Some st' -> 
+    Regs st' Rp = natToW 0.
+  Proof.
+    intros.
+    Time sym_eval ltac:(isConst) 
+      ltac:(fun ts fs => constr:(@Provers.reflexivityProver_correct ts fs)) (* prover *)
+      ltac:(composite_eval tt) (* memory evaluator *)
+      ltac:(fun ts pc st fs ps => constr:(@Demo.defaultLearnHook_correct ts fs ps)) (* unfolder *)
+      Demo.simplifier tt tt tt.
+    intuition congruence.
+  Qed.
 
-  Ltac sym_evaluator H := 
-    cbv beta iota zeta delta
-      [ sym_evalInstrs sym_evalInstr sym_evalLval sym_evalRval sym_evalLoc sym_evalStream sym_assertTest
-        sym_setReg sym_getReg
-        SepExpr.pures SepExpr.impures SepExpr.other
-        SymMem SymRegs SymPures SymVars SymUVars
-        SEP.star_SHeap SEP.liftSHeap SEP.multimap_join 
-        Expr.SemiDec_expr Expr.expr_seq_dec Expr.tvar_val_sdec Expr.Eq Expr.liftExpr
-        app map nth_error value error fold_right hd hd_error tl tail rev
-        Decidables.seq_dec 
-        DepList.hlist_hd DepList.hlist_tl 
-        SepExpr.FM.find SepExpr.FM.add SepExpr.FM.remove SepExpr.FM.map SepExpr.FM.empty SepExpr.FM.fold
-        Compare_dec.lt_eq_lt_dec nat_rec nat_rect Peano_dec.eq_nat_dec sumbool_rec sumbool_rect
-        EquivDec.equiv_dec EquivDec.nat_eq_eqdec
-        f_equal 
-        bedrock_funcs_r bedrock_types
-        fst snd
-        Env.repr Env.updateAt SEP.substV
-
-        (* remove [stateD] *)
-        stateD Expr.exprD 
-        Expr.applyD Expr.exprD Expr.Range Expr.Domain Expr.Denotation Expr.lookupAs
-        Expr.AllProvable Expr.Provable Expr.tvarD
-        SEP.sheapD SEP.starred SEP.sexprD
-        EquivDec.equiv_dec Expr.EqDec_tvar Expr.tvar_rec Expr.tvar_rect 
-        Logic.eq_sym eq_sym f_equal
-        eq_rec_r eq_rect eq_rec
-        nat_rec nat_rect
-        sumbool_rec sumbool_rect
-        
-        SEP.himp SEP.sexprD Expr.Impl 
-        Expr.applyD Expr.exprD Expr.Range Expr.Domain Expr.Denotation 
-        Expr.lookupAs
-        SepExpr.SDenotation SepExpr.SDomain
-        EquivDec.nat_eq_eqdec  
-        SEP.sheapD SEP.sepCancel
-        SepExpr.impures SepExpr.pures SepExpr.other
-        SEP.star_SHeap SEP.unify_remove_all 
-        SEP.multimap_join SEP.liftSHeap SEP.unify_remove SEP.starred 
-        Expr.tvarD Expr.Eq
-        
-        SepExpr.FM.fold SepExpr.FM.find SepExpr.FM.add SepExpr.FM.empty 
-        bedrock_types 
-                
-        Compare_dec.lt_eq_lt_dec Peano_dec.eq_nat_dec
-        SepExpr.FM.map ExprUnify.exprUnifyArgs ExprUnify.empty_Subst
-        ExprUnify.exprUnify ExprUnify.fold_left_2_opt 
-        EquivDec.equiv_dec Expr.EqDec_tvar Expr.tvar_rec Expr.tvar_rect 
-        ExprUnify.get_Eq
-        types
-(*        Provers.transitivityProverRec Provers.transitivityEqProver *) Provers.inSameGroup
-        Provers.in_seq orb
-        (*Provers.eqD*) Provers.eqD_seq
-        Expr.typeof comparator
-
-        fPlus fMinus fMult
-
-        repr_combine default footprint repr' updateAt Default_signature nil_Repr EmptySet_type SEP.Default_ssignature
-        bedrock_funcs_r bedrock_types_r
-
-        Summarize Learn Prove
-
-        symeval_read_word symeval_write_word 
-      ] in H.
-
-  Implicit Arguments istreamD [ types' ].
-
-  Module DefaultEvaluator.
-    Section with_prover.
-      Variable types : list type.
-      Variables pcT stT : tvar.
-      Variable prover : ProverT types.
-      
-      Definition symeval_read_word_default (_ : Facts prover) (_ : expr types)
-        (_ : SEP.SHeap types pcT stT) : option (expr types) :=
-        None.
-
-      Definition symeval_write_word_default (_ : Facts prover)
-        (_ : expr types) (_ : expr types) (_ : SEP.SHeap types pcT stT)
-        : option (SEP.SHeap types pcT stT) :=
-        None.
-    End with_prover.
-
-    Definition SymEvaluator_default types pcT stT : SymEvaluator types pcT stT.
-    constructor.
-    eapply symeval_read_word_default.
-    eapply symeval_write_word_default.
-    Defined.
-    
-    Definition SymEvaluator_correct_default types' (_ _ : tvar) funcs preds :     
-      @SymEvaluator_correct (repr bedrock_types_r types') funcs preds
-      (SymEvaluator_default (repr bedrock_types_r types') (tvType 0) (tvType 1)).
-    econstructor.
-      simpl; unfold symeval_read_word_default, symeval_write_word_default; simpl; congruence.
-      simpl; unfold symeval_read_word_default, symeval_write_word_default; simpl; congruence.
-    Qed.
-
-    Definition defaultLearnHook types : LearnHook types :=
-      fun _ x _ => x.
-
-    Theorem defaultLearnHook_correct types' funcs preds 
-      : @LearnHook_correct types' (@defaultLearnHook (types types')) funcs preds.
-    Proof.
-      econstructor. unfold defaultLearnHook. intros; subst; auto.
-    Qed.
-
-    Ltac simplifier H := 
-      cbv delta [ 
-        SymEvaluator_default
-        symeval_read_word_default symeval_write_word_default
-        
-        defaultLearnHook
-        reflexivityProver
-      ] in H; sym_evaluator H.
-
-    Goal forall (cs : codeSpec W (settings * state)) (stn : settings) st st' SF,
-      PropX.interp cs (SepIL.SepFormula.sepFormula SF (stn, st)) -> 
-      Structured.evalCond (RvImm (natToW 0)) IL.Eq (RvImm (natToW 0)) stn st' = Some true ->
-      evalInstrs stn st (Assign Rp (RvImm (natToW 0)) :: nil) = Some st' -> 
-      Regs st' Rp = natToW 0.
-    Proof.
-      intros.
-      Time sym_eval ltac:(isConst) 
-        ltac:(fun ts fs => constr:(@reflexivityProver_correct ts fs)) (* prover *)
-        ltac:(fun ts pc st fs ps => constr:(@SymEvaluator_correct_default ts pc st fs ps)) (* memory plugin *)
-        ltac:(fun ts pc st fs ps => constr:(@defaultLearnHook_correct ts fs ps)) (* unfolder *)
-        simplifier tt tt tt.
-      congruence.
-    Qed. 
-  End DefaultEvaluator.
-
-
-  Module PluginEvaluator.
-
-    Section evaluator.
-      Variable types : list type.
-      Variable pcT stT : tvar.
-      Variable evals : list (nat * PLUGIN.MemEval types). 
-
-      Section with_prover.
-        Variable Prover : ProverT types.
-
-
-        Section fold_first.
-          Variables T V : Type.
-          Variable F : T -> option V.
-
-          Fixpoint fold_first (ls : list T) : option V :=
-            match ls with
-              | nil => None
-              | t :: ls =>
-                match F t with
-                  | None => fold_first ls
-                  | x => x
-                end
-            end.
-        End fold_first.
-
-        Section fold_first_update.
-          Variables T : Type.
-          Variable F : T -> option T.
-
-          Fixpoint fold_first_update (ls : list T) (acc : list T) : option (list T) :=
-            match ls with
-              | nil => None
-              | t :: ls =>
-                match F t with
-                  | None => fold_first_update ls (t :: acc)
-                  | Some v => Some (rev acc ++ v :: ls)
-                end
-            end.
-        End fold_first_update.
-
-        Definition plugin_symeval_read_word (facts : Facts Prover) (p : expr types) 
-          (s : SEP.SHeap types pcT stT) : option (expr types) :=
-          let impures := SepExpr.impures s in
-          let reader i_me :=
-            let '(i,me) := i_me in
-            match FM.find i impures with
-              | Some argss =>
-                fold_first (fun args => PLUGIN.sym_read me Prover facts args p) argss
-              | None => None
-            end
-          in
-          fold_first reader evals.
-
-        Definition plugin_symeval_write_word (facts : Facts Prover) (p v : expr types)
-          (s : SEP.SHeap types pcT stT) : option (SEP.SHeap types pcT stT) :=
-          let impures := SepExpr.impures s in
-          let writer i_me :=
-          let '(i,me) := i_me in
-            match FM.find i impures with
-              | Some argss =>
-                match fold_first_update (fun args => PLUGIN.sym_write me Prover facts args p v) argss nil with
-                  | None => None
-                  | Some argss => Some (FM.add i argss impures) (** NOTE : add = replace **)
-                end
-              | None => None
-            end
-          in
-          match fold_first writer evals with
-            | None => None
-            | Some impures => Some {| impures := impures ; pures := SepExpr.pures s ; other := SepExpr.other s |}
-          end.
-      End with_prover.
-
-      Definition Plugin_SymEvaluator : SymEvaluator types pcT stT : Type :=
-      {| symeval_read_word := plugin_symeval_read_word
-       ; symeval_write_word := plugin_symeval_write_word
-       |}.
-    End evaluator.
-
-    Ltac unfolder H :=
-      cbv delta 
-        [ fold_first fold_first_update 
-          FM.find FM.add 
-          PLUGIN.sym_read PLUGIN.sym_write 
-          PLUGIN.Build_MemEval
-          plugin_symeval_read_word
-          plugin_symeval_write_word
-          Plugin_SymEvaluator
-        ] in H;
-        sym_evaluator H.
-
-    Section correctness.
-      Variable types' : list type.
-      Definition types := Env.repr bedrock_types_r types'.
-      Definition pcT := tvType 0.
-      Definition stT := tvType 1.
-      Variables tvPtr tvVal : tvar.
-      Variable funcs : functions types.
-      Variable sfuncs : SEP.sfunctions types pcT stT .
-      Variable evals : list (nat * PLUGIN.MemEval types).
-
-      Hypothesis smem_read : settings -> tvarD types tvPtr -> smem -> option (tvarD types tvVal).
-      Hypothesis smem_write : settings -> tvarD types tvPtr -> tvarD types tvVal -> smem -> option smem.
-
-      (** TODO: This is missing the necessary pre-condition to establish the connection between
-       ** [evals] and [sfuncs]
-       **)
-      Hypothesis sfuncs_evals : hlist (fun (i_me : nat * PLUGIN.MemEval types) => 
-        let (i,me) := i_me in
-        match nth_error sfuncs i with
-          | None => Empty_set
-          | Some sig => @PLUGIN.MemEval_correct _ me stT pcT tvPtr tvVal smem_read smem_write sig funcs
-        end) evals.
-
-      Definition Plugin_SymEvaluator_correct : @SymEvaluator_correct types funcs sfuncs (Plugin_SymEvaluator pcT stT evals).
-        generalize sfuncs_evals.
-        admit.
-      Qed.
-    End correctness.
-    
-  End PluginEvaluator.
-
-
-End BedrockEvaluator.
+End PluginEvaluator.
