src/sep/PtsTo2.v
@@ -1,65 +1,60 @@
 Require Import DepList List.
 Require Import Expr SepExpr SymEval.
-Require Import Memory SepIL SymIL SepTac.
-Require Import Provers.
+Require Import Memory SepIL SymIL ILTac.
+Require Import Prover.
 
 Set Implicit Arguments.
 Set Strict Implicit.
 
-Module BedrockPtsToEvaluator (P : EvaluatorPluginType BedrockHeap SepIL.ST).
-  Module Import SEP := P.SEP.
+Module BedrockPtsToEvaluator.
+  Module Import SEP := SymIL.MEVAL.SEP.
 
-  Definition pcIndex : nat := 0.
-  Definition stateIndex : nat := 1.
-  Definition pcT := tvType pcIndex.
-  Definition stT := tvType stateIndex.
+  Section hide_notation.
+    Local Notation "'pcT'" := (tvType 0).
+    Local Notation "'stT'" := (tvType 1).
+    Local Notation "'wordT'" := (tvType 0).
+    Local Notation "'ptrT'" := (tvType 0).
 
-  Definition ptsto32_types_r : Env.Repr Expr.type :=
-  {| Env.footprint := 
-    ((0, {| Impl := W 
-          ; Eq := seq_dec |}) ::
-     (1, {| Impl := IL.settings * IL.state
-          ; Eq := fun _ _ => None
-          |}) :: nil) :: nil
-   ; Env.default := EmptySet_type 
-   |}.
+    Definition ptsto32_types_r : Env.Repr Expr.type :=
+    {| Env.footprint := 
+       ((0, {| Impl := W 
+             ; Eq := seq_dec |}) ::
+        (1, {| Impl := IL.settings * IL.state
+             ; Eq := fun _ _ => None
+             |}) :: nil) :: nil
+     ; Env.default := EmptySet_type 
+     |}.
 
+    Section parametric.
+      Variable types : list type.
+      Variable Prover : ProverT types.
 
-  Definition wordIndex := 0.
-  Definition ptrIndex := 0.
+      Definition psummary := Facts Prover.
 
-  Section parametric.
-    Variable types : list type.
-    Variable Prover : ProverT types.
-
-
-    Definition psummary := Facts Prover.
-
-    Definition expr_equal (sum : psummary) (tv : tvar) (a b : expr types) : bool :=
-      match seq_dec a b with
-        | Some _ => true
-        | None => 
-          Provers.Prove Prover sum (Equal tv a b)
+      Definition expr_equal (sum : psummary) (tv : tvar) (a b : expr types) : bool :=
+        match seq_dec a b with
+          | Some _ => true
+          | None => Prove Prover sum (Equal tv a b)
       end.
     
-    Definition sym_read_word_ptsto32 (summ : psummary) (args : list (expr types)) (p : expr types) 
-      : option (expr types) :=
-      match args with
-        | p' :: v' :: nil => 
-          if expr_equal summ (tvType ptrIndex) p p' then Some v' else None
-        | _ => None
-      end.
-    Definition sym_write_word_ptsto32 (summ : psummary) (args : list (expr types)) (p v : expr types)
-      : option (list (expr types)) :=
-      match args with
-        | p' :: v' :: nil =>
-          if expr_equal summ (tvType ptrIndex) p p' then Some (p :: v :: nil) else None
-        | _ => None
-      end.
+      Definition sym_read_word_ptsto32 (summ : psummary) (args : list (expr types)) (p : expr types) 
+        : option (expr types) :=
+        match args with
+          | p' :: v' :: nil => 
+            if expr_equal summ ptrT p p' then Some v' else None
+          | _ => None
+        end.
+      Definition sym_write_word_ptsto32 (summ : psummary) (args : list (expr types)) (p v : expr types)
+        : option (list (expr types)) :=
+        match args with
+          | p' :: v' :: nil =>
+            if expr_equal summ ptrT p p' then Some (p :: v :: nil) else None
+          | _ => None
+        end.
   End parametric.
 
-  Definition MemEval_ptsto32 types : @P.MemEval types.
-  eapply P.Build_MemEval.
+  Definition MemEval_ptsto32 types : @MEVAL.Plugin.MemEvalPred types.
+  eapply MEVAL.Plugin.Build_MemEvalPred.
   eapply sym_read_word_ptsto32.
   eapply sym_write_word_ptsto32.
   Defined.
@@ -68,213 +63,150 @@ Module BedrockPtsToEvaluator (P : EvaluatorPluginType BedrockHeap SepIL.ST).
     Variable types' : list type.
     Definition types := Env.repr ptsto32_types_r types'.
 
+    Local Notation "'pcT'" := (tvType 0).
+    Local Notation "'stT'" := (tvType 1).
+    Local Notation "'wordT'" := (tvType 0).
+    Local Notation "'ptrT'" := (tvType 0).
+
     Definition ptsto32_ssig : ssignature types pcT stT.
     refine (
-      {| SepExpr.SDomain := tvType ptrIndex :: tvType wordIndex :: nil
+      {| SepExpr.SDomain := ptrT :: wordT :: nil
        ; SepExpr.SDenotation := _
        |}).
     refine (ptsto32 _).
     Defined.
-(*
+
     Variable funcs : functions types.
+    Variable Prover : ProverT types.
     Variable Prover_correct : ProverT_correct Prover funcs.
 
     Theorem expr_equal_correct : 
-      forall (sum : psummary) (tv : tvar) (a b : expr types),
-        expr_equal sum tv a b = true ->
+      forall (sum : Facts Prover) (tv : tvar) (a b : expr types),
+        expr_equal Prover sum tv a b = true ->
         forall uvars vars,
-          Provers.Valid Prover_correct uvars vars sum ->
+          Valid Prover_correct uvars vars sum ->
           match exprD funcs uvars vars a tv , exprD funcs uvars vars b tv with 
             | Some l , Some r => l = r
             | _ , _ => True
           end.
     Proof.
       unfold expr_equal. intros. destruct (seq_dec a b); subst.
-      destruct (exprD funcs uvars vars0 b tv); auto.
+      destruct (exprD funcs uvars vars b tv); auto.
       generalize (Prove_correct Prover_correct). intro XX; apply XX in H0; clear XX.
-      eapply H0 in H. unfold Provable in H. simpl in H. (*
-      case_eq (exprD funcs uvars vars0 a tv); auto.
-      case_eq (exprD funcs uvars vars0 b tv); auto. intros.
-      unfold ValidExp in *. apply H1 in H; eauto. clear H1.
-      destruct H.
-      cutrewrite (x = tv) in H.
-      rewrite H2 in *. rewrite H3 in *. auto.
+      case_eq (exprD funcs uvars vars a tv); auto.
+      case_eq (exprD funcs uvars vars b tv); auto.
+      intros; eapply H0 in H. unfold Provable in H. simpl in H. 
+      intros. rewrite H1 in *. rewrite H2 in *. auto. 
 
-      revert H0.
-      case_eq (exprD funcs uvars vars0 a x); intros; try contradiction.
-      assert (exprD funcs uvars vars0 a x <> None) by congruence.
-      assert (exprD funcs uvars vars0 a tv <> None) by congruence.
-      eapply exprD_det; eauto.
-      rewrite H0 in *. contradiction.      
-    Qed.*)
-    Admitted.
+      unfold ValidProp. simpl. rewrite H1. rewrite H2. eauto.
+    Qed.
 
+    Ltac expose :=
+      repeat (
+        match goal with 
+          | [ H : match applyD _ _ ?A _ _ with
+                    | Some _ => _ 
+                    | None => False 
+                  end |- _ ] =>
+          destruct A; simpl in H; try (exfalso; assumption)
+          | [ H : context [ match exprD ?A ?B ?C ?D ?E with
+                              | None => _
+                              | Some _ => _
+                            end ] |- _ ] =>
+          revert H; case_eq (exprD A B C D E); simpl; intros; 
+            try (exfalso; assumption)
+          | [ H : context [ match expr_equal ?A ?B ?C ?D with
+                              | true => _
+                              | false => _
+                            end ] |- _ ] =>
+          revert H; case_eq (expr_equal A B C D); intros; 
+            try (exfalso; congruence)
+          | [ H : expr_equal ?A ?B ?C ?D = true 
+            , H' : AllProvable _ _ _ ?A |- _ ] =>
+          generalize (@expr_equal_correct _ _ _ _ H _ _ H'); clear H; intros
+          | [ H : Some _ = Some _ |- _ ] =>
+            inversion H; clear H; subst
+          | [ H : exprD _ _ _ _ _ = Some _ |- _ ] =>
+            rewrite H in *
+        end; simpl in * ).
 
-  Ltac expose :=
-    repeat (unfold wordIndex, ptrIndex in *; 
-            match goal with 
-              | [ H : match applyD _ _ ?A _ _ with
-                        | Some _ => _ 
-                        | None => False 
-                      end |- _ ] =>
-              destruct A; simpl in H; try (exfalso; assumption)
-              | [ H : context [ match exprD ?A ?B ?C ?D ?E with
-                          | None => _
-                          | Some _ => _
-                        end ] |- _ ] =>
-              revert H; case_eq (exprD A B C D E); simpl; intros; 
-                try (exfalso; assumption)
-              | [ H : context [ match expr_equal ?A ?B ?C ?D with
-                                  | true => _
-                                  | false => _
-                                end ] |- _ ] =>
-                revert H; case_eq (expr_equal A B C D); intros; 
-                  try (exfalso; congruence)
-              | [ H : expr_equal ?A ?B ?C ?D = true 
-                , H' : AllProvable _ _ _ ?A |- _ ] =>
-                generalize (@expr_equal_correct _ _ _ _ H _ _ H'); clear H; intros
-              | [ H : Some _ = Some _ |- _ ] =>
-                inversion H; clear H; subst
-              | [ H : exprD _ _ _ _ _ = Some _ |- _ ] =>
-                rewrite H in *
-            end; simpl in * ).
+    Lemma sym_read_ptsto32_correct : forall args uvars vars cs summ pe p ve m stn,
+      sym_read_word_ptsto32 Prover summ args pe = Some ve ->
+      Valid Prover_correct uvars vars summ ->
+      exprD funcs uvars vars pe ptrT = Some p ->
+      match 
+        applyD (exprD funcs uvars vars) (SDomain ptsto32_ssig) args _ (SDenotation ptsto32_ssig)
+        with
+        | None => False
+        | Some p => ST.satisfies cs p stn m
+      end ->
+      match exprD funcs uvars vars ve wordT with
+        | Some v =>
+          ST.HT.smem_get_word (IL.implode stn) p m = Some v
+        | _ => False
+      end.
+    Proof.
+      simpl; intros.
+      unfold sym_read_word_ptsto32 in H.
+      repeat (destruct args; try congruence).
+      revert H.
+      case_eq (expr_equal Prover summ ptrT pe e); try congruence.
+      intros.
+      inversion H3; clear H3; subst.
+      eapply expr_equal_correct in H; eauto.
+      simpl applyD in H2.
+      expose; try congruence.
+      unfold ST.satisfies in H6. PropXTac.propxFo. 
+    Qed.
 
-  Lemma sym_read_ptsto32_correct : forall args uvars vars cs summ pe p ve m stn,
-    sym_read_word_ptsto32 summ args pe = Some ve ->
-    Provers.Valid Prover_correct uvars vars summ ->
-    exprD funcs uvars vars pe (tvType ptrIndex) = Some p ->
-    match 
-      applyD (exprD funcs uvars vars) (SDomain ptsto32_ssig) args _ (SDenotation ptsto32_ssig)
-      with
-      | None => False
-      | Some p => ST.satisfies cs p stn m
-    end ->
-    match exprD funcs uvars vars ve (tvType wordIndex) with
-      | Some v =>
-        ST.HT.smem_get_word (IL.implode stn) p m = Some v
-      | _ => False
-    end.
-  Proof.
-    simpl; intros.
-    unfold sym_read_word_ptsto32 in H.
-    repeat (destruct args; try congruence).
-    revert H.
-    case_eq (expr_equal summ (tvType ptrIndex) pe e); try congruence.
-    intros.
-    inversion H3; clear H3; subst.
-    eapply expr_equal_correct in H; eauto.
-    simpl applyD in H2.
-    expose; try congruence.
-    unfold ST.satisfies in H6. PropXTac.propxFo. 
-  Qed.
+    Lemma sym_write_word_ptsto32_correct : forall args uvars vars cs summ pe p ve v m stn args',
+      sym_write_word_ptsto32 Prover summ args pe ve = Some args' ->
+      Valid Prover_correct uvars vars summ ->
+      exprD funcs uvars vars pe ptrT = Some p ->
+      exprD funcs uvars vars ve wordT = Some v ->
+      match
+        applyD (@exprD _ funcs uvars vars) (SDomain ptsto32_ssig) args _ (SDenotation ptsto32_ssig)
+        with
+        | None => False
+        | Some p => ST.satisfies cs p stn m
+      end ->
+      match 
+        applyD (@exprD _ funcs uvars vars) (SDomain ptsto32_ssig) args' _ (SDenotation ptsto32_ssig)
+        with
+        | None => False
+        | Some pr => 
+          match ST.HT.smem_set_word (IL.explode stn) p v m with
+            | None => False
+            | Some sm' => ST.satisfies cs pr stn sm'
+          end
+      end.
+    Proof.
+      simpl; intros; expose.
+      revert H; case_eq (expr_equal Prover summ ptrT pe e); intros; try congruence.
+      inversion H6; clear H6; subst. simpl.
+      rewrite H1. rewrite H2.
+      
+      case_eq (smem_set_word (IL.explode stn) p v m); intros; unfold ptsto32 in *. 
+      PropXTac.propxFo.
+      eapply smem_set_get_word_eq; eauto.
+      eapply IL.implode_explode.
+      eapply expr_equal_correct in H; eauto.
+      rewrite H1 in H. rewrite H3 in H. subst.
+      unfold ST.satisfies in H5. PropXTac.propxFo.
+      eapply smem_set_get_valid_word; eauto.
+    Qed.  
 
-  Lemma sym_write_word_ptsto32_correct : forall args uvars vars cs summ pe p ve v m stn args',
-    sym_write_word_ptsto32 summ args pe ve = Some args' ->
-    Provers.Valid Prover_correct uvars vars summ ->
-    exprD funcs uvars vars pe (tvType ptrIndex) = Some p ->
-    exprD funcs uvars vars ve (tvType wordIndex) = Some v ->
-    match
-      applyD (@exprD _ funcs uvars vars) (SDomain ptsto32_ssig) args _ (SDenotation ptsto32_ssig)
-      with
-      | None => False
-      | Some p => ST.satisfies cs p stn m
-    end ->
-    match 
-      applyD (@exprD _ funcs uvars vars) (SDomain ptsto32_ssig) args' _ (SDenotation ptsto32_ssig)
-      with
-      | None => False
-      | Some pr => 
-        match ST.HT.smem_set_word (IL.explode stn) p v m with
-          | None => False
-          | Some sm' => ST.satisfies cs pr stn sm'
-        end
-    end.
-  Proof.
-    simpl; intros; expose.
-
-    unfold ST.satisfies in *. PropXTac.propxFo. 
-    case_eq (smem_set_word (IL.explode stn) p v m).
-    intros. unfold ptsto32. PropXTac.propxFo.
-    eapply smem_set_get_word_eq; eauto.
-    eapply IL.implode_explode.
-    eapply expr_equal_correct in H; eauto.
-    rewrite H1 in H. rewrite H3 in H. subst.
-    eapply smem_set_get_valid_word; eauto.
-  Qed.  
-
-*)
   End correctness.
 
   Definition MemEval_ptsto32_correct types' funcs
-    : @P.MemEval_correct _ (MemEval_ptsto32 (Env.repr ptsto32_types_r types')) (tvType 1) (tvType 0) (tvType 0) (tvType 0)
-    SepTac.smem_read SepTac.smem_write (ptsto32_ssig types') funcs.
-(*
-  eapply P.Build_MemEval_correct;
-    simpl; unfold MemEval_ptsto32; try (rewrite P.proj_sym_read || rewrite P.proj_sym_write);
-  simpl in *; intros; (eapply (@sym_read_ptsto32_correct types') || eapply (@sym_write_word_ptsto32_correct types')); eauto.
-  Qed.
-*)
+    : @MEVAL.Plugin.MemEvalPred_correct _ (MemEval_ptsto32 (Env.repr ptsto32_types_r types')) (tvType 0) (tvType 1) (IL.settings * IL.state) (tvType 0) (tvType 0)
+    (@IL_mem_satisfies types') (@IL_ReadWord types') (@IL_WriteWord types') (ptsto32_ssig types') funcs.
+  Proof.
+    eapply MEVAL.Plugin.Build_MemEvalPred_correct;
+      simpl; unfold MemEval_ptsto32, IL_ReadWord, IL_WriteWord, IL_mem_satisfies, IL.ReadWord, IL.WriteWord.
+    destruct stn_st; simpl in *.
+    (** TODO: the interface is wrong, it needs to be over the symbolic memory **)
   Admitted.
+  End hide_notation.
 
 End BedrockPtsToEvaluator.
-
-(*
-Module DEMO := BedrockPtsToEvaluator SymIL.PLUGIN.
-
-Import BedrockEvaluator.
-
-
-Record mem_evaluator : Type :=
-{ READER : _ 
-; WRITER : _
-; CORRECTNESS : BedrockEvaluator.Correctness READER WRITER
-}.
-
-(** TODO: I need to find some way to build this using tactics! **)
-Definition ptsto_evaluator : mem_evaluator.
-refine (
-  {| READER := fun typs summ p s =>
-    match FM.find 0 (impures s) with
-      | None => None
-      | Some argss =>
-        @fold_args unit (fun _ => unit) (bedrock_types ++ typs) (expr (bedrock_types ++ typs)) 
-          (fun _ _ args =>
-            match args with
-              | p' :: v' :: nil => 
-                if DEMO.expr_equal _ summ (tvType 0) p p' then Some v' else None
-              | _ => None
-            end)
-          tt tt argss
-    end
-   ; WRITER := fun typs summ p v s => 
-     match FM.find 0 (impures s) with
-      | None => None
-      | Some argss =>
-        let res :=
-          @fold_args_update unit (fun _ => unit) (bedrock_types ++ typs)
-            (fun _ _ args =>
-              match args with
-                | p' :: v' :: nil => 
-                  if DEMO.expr_equal _ summ (tvType 0) p p' then Some (p' :: v :: nil) else None
-                | _ => None
-              end)
-            tt tt argss
-        in
-        match res with
-          | None => None
-          | Some res =>
-            Some {| impures := FM.add 0 res (impures s) ; pures := pures s ; other := other s |}
-        end
-    end
-   ; CORRECTNESS := 
-     {| TypeImage := nil
-      ; FuncImage := fun _ => nil
-      ; PredImage := fun t => (0, DEMO.ptsto32_ssig t) :: nil
-      ; ReadCorrect := _
-      ; WriteCorrect := _
-      |}
-   |}); unfold READER, WRITER.
-admit.
-admit.
-Defined.
-*)
